Experiments/ProofChecking/Combined.lean
@@ -1,0 +1,338 @@
+/-
+
+A combined LSR parser and checker.
+
+Cayden Codel
+Carnegie Mellon University
+
+-/
+
+import LeanSAT.Data.Cnf
+import LeanSAT.Data.Literal
+import LeanSAT.Data.ICnf
+
+import LeanSAT.Model.PropFun
+
+import Experiments.ProofChecking.PPA
+import Experiments.ProofChecking.PS
+import Experiments.ProofChecking.RangeArray
+
+import LeanSAT.Solver.Dimacs
+
+open LeanSAT LeanSAT.Model PropFun Except
+
+namespace SR
+
+@[specialize]
+class Formula (F : Type _) where
+  size : F → Nat
+  empty : F
+  addClause : F → IClause → F
+  deleteClause : F → Nat → F
+  isDeleted : F → Nat → Bool
+  foldMOnClause : F → Nat →
+    {β : Type v} → {m : Type v → Type w} → [Monad m] →
+    (f : β → ILit → m β) → (init : β) → m β
+  -- Technically, `toPropFun` can be defined in terms of foldMOnClause
+  --toPropFun : F → PropFun IVar
+
+open Formula in
+class LawfulFormula (F : Type _) [Formula F] where
+  size_empty : size (empty : F) = 0
+  size_addClause (f : F) (c : IClause) : size (addClause f c) = size f + 1
+  size_deleteClause (f : F) (i : Nat) : size (deleteClause f i) = size f
+  /-- All clauses out-of-bounds are deleted. -/
+  isDeleted_ge_size (f : F) (i : Nat) : i ≥ size f → isDeleted f i = false
+  /-- If we delete a clause, it should actually be marked as deleted. -/
+  isDeleted_deleteClause (f : F) (i j : Nat) : isDeleted (deleteClause f i) j =
+    if i = j then true else isDeleted f j
+  /-- Added clauses are, by default, not deleted. -/
+  isDeleted_addClause (f : F) (c : IClause) (i : Nat) : isDeleted (addClause f c) (size f) = false
+  /-- Folding across a just-deleted clause should give back init. -/
+  foldlMOnClause_deleteClause (f : F) (i : Nat) {β : Type v} {m : Type v → Type w} [Monad m]
+    (g : β → ILit → m β) (init : β) : foldMOnClause (deleteClause f i) i g init = pure init
+  /-- If we fold after adding, it's the same as folding across either a clause in the formula,
+      or the clause we just added. -/
+  foldlMOnClause_addClause (f : F) (c : IClause) (i : Nat) {β : Type v} {m : Type v → Type w} [Monad m]
+    (g : β → ILit → m β) (init : β) : foldMOnClause (addClause f c) i g init =
+      if i = size f then c.foldlM g init else foldMOnClause f i g init
+
+instance : Formula (RangeArray ILit) where
+  size := RangeArray.size
+  empty := RangeArray.empty
+  addClause := RangeArray.add
+  deleteClause := RangeArray.delete
+  isDeleted := RangeArray.isDeleted
+  foldMOnClause := fun F i _ _ _ f init => F.foldlM_index f init i
+
+structure SRLine where
+  clause : IClause
+  witness_lits : Array ILit
+  witness_maps : Array (IVar × ILit)
+  up_hints : Array Nat                -- Already 0-indexed clause IDs into the accumulated formula
+  rat_hints : Array (Nat × Array Nat) -- Already 0-indexed clause IDs into the accumulated formula
+
+structure SRDeletionLine where
+  clauses : Array Nat
+
+-- TODO: Move to LeanSAT
+-- CC: James claims that CPS is easier to reason about and is more performant,
+--     and Mario claims that Except blobbies are expensive for Lean to constantly create.
+--     Make a `call/cc` construct later?
+def parseLit (maxVar : Nat) (C : IClause) (s : String) : Except (Except String IClause) IClause := do
+  match s.toInt? with
+  | none => throw (throw s!"Literal is not a number: {s}")
+  | some n =>
+    if hn : n = 0 then
+      throw (return C)
+    else
+      if n.natAbs > maxVar then
+        throw (throw s!"Literal {n} is greater than the maximum variable {maxVar}")
+      else
+        if n < 0 then
+          return C.push ⟨n, hn⟩
+        else
+          return C.push ⟨n, hn⟩
+
+-- CC: Move to LeanSAT/replace the existing `parseClause`
+def parseClause {CNF : Type _} [Formula CNF] (maxVar : Nat) (F : CNF) (s : String) : Except String CNF :=
+  match s.splitOn " " |>.foldlM (parseLit maxVar) #[] with
+  | ok _ => throw "Zero not encountered on this line"
+  | error e =>
+    match e with
+    | ok c => return Formula.addClause F c
+    | error e => throw e
+
+-- CC: Can be made into a state machine later, to consume tokens rather than whole lines
+--     Otherwise, parsing can take up a lot of CPU time.
+--     (Plus, streaming?)
+-- Parses the CNF given a string and an empty formula to read the clauses into
+def parseFormula {CNF : Type _} [Formula CNF] (s : String) (F : CNF) : Except String (Nat × CNF) := do
+  -- CC: See SRParser.lean for a more idiomatic version. Had trouble with universe levels
+  match s.splitOn "\n" |>.filter (fun line => !line.startsWith "c" && line.any (!·.isWhitespace)) with
+  | [] => throw "Empty formula"
+  | (pLine :: clauseLines) =>
+
+  /-
+  Doing (nvars, ncls) ← Solver.Dimacs.parseHeader pLine gives
+
+  stuck at solving universe constraint
+  u =?= max ?u.3706 ?u.3707
+while trying to unify
+  (?m.3712 s F pLine clauseLines × ?m.3713 s F pLine clauseLines) (?m.3712 s F pLine clauseLines)
+    (?m.3713 s F pLine clauseLines)
+with
+  (?m.3712 s F pLine clauseLines × ?m.3713 s F pLine clauseLines) (?m.3712 s F pLine clauseLines)
+    (?m.3713 s F pLine clauseLines)
+  -/
+
+    match Solver.Dimacs.parseHeader pLine with
+    | error s => throw s
+    | ok (nvars, ncls) =>
+      let F ← clauseLines.foldlM (parseClause nvars) F
+      if Formula.size F != ncls then
+        throw s!"Expected {ncls} clauses, but found {Formula.size F}"
+      else
+        return (nvars, F)
+
+-- CC: In some sense, the witness can be assumed right away (and maybe even the negation of the candidate clause)
+--     But for a clean separation of parsing and checking, we store in an intermediate data structure.
+inductive SRParsingMode
+| clause
+| witness_tf
+| witness_mapped_ready
+| witness_mapped_halfway : IVar → SRParsingMode
+| up_hints
+| rat_hints : Nat × Array Nat → SRParsingMode
+| done_with_line -- Could be removed, in favor of Except (Except String SRLine), but this is arguably more elegant
+deriving BEq
+
+open SRParsingMode
+
+def parseSRAtom (pivot : Option ILit) (p : SRLine × SRParsingMode) (s : String) : Except String (SRLine × SRParsingMode) :=
+  let ⟨line, mode⟩ := p
+  -- No matter what, the string should be a number, so parse it as an int
+  match s.toInt? with
+  | none => throw s!"Atom {s} didn't parse to a number"
+  | some n =>
+    if hn : n = 0 then
+      match mode with
+      | .clause =>
+        -- We don't have a witness, so we insert the pivot into the witness and continue, if the clause isn't empty
+        match pivot with
+        | none => return ⟨line, .up_hints⟩
+        | some pivot => return ⟨{ line with witness_lits := line.witness_lits.push pivot }, .up_hints⟩
+      | .witness_tf => return ⟨line, .up_hints⟩
+      | .witness_mapped_ready => return ⟨line, .up_hints⟩
+      | .witness_mapped_halfway _ => throw s!"Only got half a substitution mapping when ending a witness"
+      | .up_hints => return ⟨line, .done_with_line⟩
+      | .rat_hints hints => return ⟨{ line with rat_hints := line.rat_hints.push hints }, .done_with_line⟩
+      | .done_with_line => throw s!"Addition line continued after last ending 0"
+    else
+      match mode with
+      | .clause =>
+        match pivot with
+        | none => throw "No pivot provided for the clause"
+        | some pivot =>
+          if n = pivot.val then
+            -- Seeing the pivot again means we're parsing a witness
+            return ⟨{ line with witness_lits := line.witness_lits.push ⟨n, hn⟩ }, .witness_tf⟩
+          else
+            -- It's not the pivot (and it's not 0), so add it to the clause
+            return ⟨{ line with clause := line.clause.push ⟨n, hn⟩ }, .clause⟩
+      | .witness_tf =>
+        match pivot with
+        | none => throw "No pivot provided for the witness"
+        | some pivot =>
+          if n = pivot.val then
+            -- Seeing the pivot again means we're parsing the substitution mappings
+            return ⟨line, .witness_mapped_ready⟩
+          else
+            return ⟨{ line with witness_lits := line.witness_lits.push ⟨n, hn⟩ }, .witness_tf⟩
+      | .witness_mapped_ready =>
+        match pivot with
+        | none => throw "No pivot provided for the witness"
+        | some pivot =>
+          if n = pivot.val then
+            throw s!"Saw pivot again in substitution mapping"
+          else
+            if n < 0 then
+              throw s!"First of a substitution mapping must be positive"
+            else
+              return ⟨line, .witness_mapped_halfway ⟨n.natAbs, Int.natAbs_pos.mpr hn⟩⟩
+      | .witness_mapped_halfway v =>
+        return ⟨{line with witness_maps := line.witness_maps.push ⟨v, ⟨n, hn⟩⟩ }, .witness_mapped_ready⟩
+      | .up_hints =>
+        if n < 0 then
+          match pivot with
+          | none => throw "Can't have RAT hints for empty clauses"
+          | _ =>
+            -- This is our first RAT hint - start building it
+            return ⟨line, .rat_hints ⟨n.natAbs - 1, #[]⟩⟩
+        else
+          return ⟨{ line with up_hints := line.up_hints.push (n.natAbs - 1) }, .up_hints⟩
+      | .rat_hints ⟨h, hints⟩ =>
+        if n < 0 then
+          -- This is a new RAT hint - add the old one
+          return ⟨{ line with rat_hints := line.rat_hints.push ⟨h, hints⟩ }, .rat_hints ⟨n.natAbs - 1, #[]⟩⟩
+        else
+          return ⟨line, .rat_hints ⟨h, hints.push (n.natAbs - 1)⟩⟩
+      | .done_with_line => throw s!"Addition line continued after last ending 0"
+
+def parseLSRLine (maxId : Nat) (s : String) : Except String (Nat × (SRLine ⊕ SRDeletionLine)) :=
+  match s.splitOn " " with
+  | [] => throw "Empty line"
+  | [_] => throw s!"Single atom line: {s}, with id {maxId}"
+  | (id :: hd :: tls) =>
+    match hd with
+    | "d" =>
+      -- Check to make sure the maxId is (non-strictly) monotonically increasing
+      match id.toNat? with
+      | none => throw "Line ID is not a number"
+      | some id =>
+        if id < maxId then
+          throw "Deletion line id is not increasing"
+        else
+          match tls.foldlM (fun arr str =>
+            match str.toNat? with
+            | none => throw (throw s!"{str} was not a number")
+            | some 0 => throw (return arr)
+            | some (n + 1) => return arr.push n) #[] with
+          | ok _ => throw "Zero not found on deletion line"
+          | error e => return ⟨max id maxId, .inr (SRDeletionLine.mk (← e))⟩
+    | _ =>
+      -- We have an addition line, so the maxId should strictly increase
+      match id.toNat? with
+      | none => throw "Line ID is not a number"
+      | some id =>
+        if id ≤ maxId then
+          throw s!"Addition line id is not increasing: parsed {id}, max {maxId}"
+        else
+          match hd.toInt? with
+          | none => throw "Pivot is not a number"
+          | some n =>
+            let line : SRLine := ⟨#[], #[], #[], #[], #[]⟩
+            if hn : n = 0 then
+              match tls.foldlM (parseSRAtom none) ⟨line, .up_hints⟩ with
+              | error str => throw str
+              | ok ⟨line, mode⟩ =>
+                if mode != .done_with_line then
+                  throw "Addition line for empty clause didn't end with 0"
+                else
+                  return ⟨id, .inl line⟩
+            else
+              match tls.foldlM (parseSRAtom (some ⟨n, hn⟩)) ⟨{ line with clause := line.clause.push ⟨n, hn⟩ }, .clause⟩ with
+              | error str => throw str
+              | ok ⟨line, mode⟩ =>
+                if mode != .done_with_line then
+                  throw "Addition line didn't end with 0"
+                else
+                  return ⟨id, .inl line⟩
+
+--------------------------------------------------------------------------------
+
+@[specialize]
+def checkLine {CNF : Type _} [Formula CNF] (F : CNF) (τ : PPA) (σ : PS)
+  (clause : IClause) (w_lits : Array ILit) (w_maps : Array (IVar × ILit))
+  (up_hints : Array Nat) (rat_hints : Array (Nat × Array Nat)) : Except Bool (CNF × PPA × PS) :=
+    --(success : CNF → PPA → PS → Except Bool )
+    --(fail : String → α) : α :=
+    error false
+
+--------------------------------------------------------------------------------
+end SR
+
+open SR SR.Formula
+
+inductive SRResult where
+  | err   : SRResult -- Some kind of error
+  | valid : SRResult -- Didn't derive the empty clause
+  | unsat : SRResult
+
+@[specialize]
+def checkLines {CNF : Type _} [Formula CNF] (F : CNF) (τ : PPA) (σ : PS) : List String → SRResult
+  | [] => SRResult.valid
+  | line :: lines =>
+    match SR.parseLSRLine (size F) line with
+    | Except.error str =>
+      dbg_trace str
+      SRResult.err
+
+    -- TODO: maxId logic
+    | Except.ok (_, Sum.inl ⟨c, wl, wm, uh, rh⟩) =>
+      match SR.checkLine F τ σ c wl wm uh rh with
+      | Except.error true => SRResult.err
+      | Except.error false => SRResult.err
+      | Except.ok (F, τ, σ) => checkLines F τ σ lines
+    | Except.ok (_, Sum.inr l) =>
+      checkLines (l.clauses.foldl Formula.deleteClause F) τ σ lines
+
+def main (args : List String) : IO Unit := do
+  if args.length != 2 then
+    IO.println "Usage: ./exe <cnf-file> <lsr-file>"
+    return
+
+  let cnfFile := args[0]!
+  let lsrFile := args[1]!
+  let contents ← IO.FS.withFile cnfFile .read (·.readToEnd)
+  let (nvars, F) ← IO.ofExcept <| SR.parseFormula contents (RangeArray.empty : RangeArray ILit)
+  let numClauses := F.size
+  IO.println s!"c Formula has {numClauses} clauses and {nvars} variables"
+
+  let lsrContents ← IO.FS.withFile lsrFile .read (·.readToEnd)
+  let lsrLinesRaw := lsrContents.splitOn "\n"
+      |>.filter (fun line => !line.startsWith "c" && line.any (!·.isWhitespace))
+
+  let numLines := lsrLinesRaw.length
+  --let lineFailed : String → IO Unit := fun str =>
+  --  IO.println s!"c Line failed: {str}"
+
+  match @checkLines (RangeArray ILit) _ F (PPA.new (nvars * 2)) (PS.new (nvars * 2)) lsrLinesRaw with
+  | .valid =>
+    IO.println "c Proof was valid, but did not derive the empty clause"
+    IO.println "s VERIFIED"
+  | .err =>
+    IO.println "c Proof failed"
+    IO.println "s INVALID"
+  | .unsat =>
+    IO.println "s VERIFIED UNSAT"
