Experiments/ProofChecking/SRCheckerBasic.lean
@@ -1,0 +1,216 @@
+/-
+
+An LSR checker for the RangeArray data structure.
+
+Author: Cayden Codel
+Carnegie Mellon University
+
+-/
+
+import Experiments.ProofChecking.PPA
+import Experiments.ProofChecking.PS
+import Experiments.ProofChecking.RangeArray
+import Experiments.ProofChecking.SRParserBasic
+
+import LeanSAT.Data.Cnf
+import LeanSAT.Data.ICnf
+import LeanSAT.Model.PropFun
+import LeanSAT.Model.Subst
+
+open LeanSAT LeanSAT.Model Nat
+open PPA PS LitVar ILit IVar LawfulLitVar PropFun
+open Except
+
+namespace SR
+
+-- Apply unit propagation to clause `i`.
+@[inline, always_inline]
+def unitProp (τ : PPA) (F : RangeArray ILit) (i : Nat) : MUPResult :=
+  unitPropOnIndexes τ F.data (F.index i) (F.index i + F.rsize i)
+
+@[inline, always_inline]
+def reduce (σ : PS) (F : RangeArray ILit) (i : Nat) : ReductionResult :=
+  σ.reduceOnIndexes F.data (F.index i) (F.index i + F.rsize i)
+
+-- On error: The Bool being true indicates contradiction, false indicates actual error.
+@[inline]
+def applyUPHint (F : RangeArray ILit) (bumps : Nat) (τ : PPA) (hint : Nat) : Except (PPA × Bool) PPA :=
+  if hint < F.size && !F.isDeleted hint then
+    match unitProp τ F hint with
+    | .falsified => error ⟨τ, true⟩
+    | .satisfied =>
+      -- dbg_trace s!"ERROR: UP found a satisfied clause at index {hint}"
+      error ⟨τ, false⟩
+    | .multipleUnassignedLiterals =>
+      -- dbg_trace s!"ERROR: UP found a non-unit clause at index {hint}"
+      error ⟨τ, false⟩
+    | .unit l =>
+      -- dbg_trace s!"    Hint {hint} makes clause unit on literal {l}"
+      ok (τ.setLitFor l bumps)
+  else
+    -- dbg_trace s!"ERROR: Hint out of bounds"
+    error ⟨τ, false⟩
+
+@[inline, always_inline]
+def applyUPHints (F : RangeArray ILit) (offset : Nat) (τ : PPA) (hints : Array Nat) : Except (PPA × Bool) PPA :=
+  -- A re-implementation of hints.foldlM ..., except it uses an explicit
+  -- index and is tail-recursive in its loop.
+  let rec go (i : Nat) (τ : PPA) : Except (PPA × Bool) PPA :=
+    if hi : i < hints.size then
+      match applyUPHint F offset τ (hints.get ⟨i, hi⟩) with
+      | ok τ => go (i + 1) τ
+      | error ⟨τ, true⟩ => error ⟨τ, true⟩
+      | error ⟨τ, false⟩ => error ⟨τ, false⟩
+    else ok τ
+  termination_by hints.size - i
+  go 0 τ
+  --hints.foldlM (init := τ) (applyUPHint F offset)
+
+-- Scans the RAT hints
+def scanRATHints (clauseId : Nat) (ratHintIndexes : Array Nat) : Option (Fin ratHintIndexes.size) :=
+  match ratHintIndexes.foldlM (init := 0) (fun counter hint =>
+        if hint = clauseId then error counter
+        else ok (counter + 1)) with
+  | ok _ => none
+  | error index =>
+    if hi : index < ratHintIndexes.size then some ⟨index, hi⟩
+    else none
+
+-- Finds the RAT hint pair that matches the clauseId
+def findRATHintIndex (ratIndex clauseId : Nat) (ratHintIndexes : Array Nat) : Option (Fin ratHintIndexes.size) :=
+  -- If the RAT hints are sorted, then check the one under our "cached pointer" first
+  if h_index : ratIndex < ratHintIndexes.size then
+    let ratClauseIndex := ratHintIndexes.get ⟨ratIndex, h_index⟩
+    if ratClauseIndex = clauseId then some ⟨ratIndex, h_index⟩
+    else scanRATHints clauseId ratHintIndexes
+  else
+    scanRATHints clauseId ratHintIndexes
+
+-- Returns an updated PPA. Bool is true if the clause is satisfied by σ or τ, false otherwise.
+def assumeRATClause (F : RangeArray ILit) (index : Fin F.size) (σ : PS) (τ : PPA) : PPA × Bool :=
+  let size := F.rsize index
+  let rec go (i : Nat) (τ : PPA) : PPA × Bool :=
+    if hi : i < size then
+      let lit := F.getOffset index ⟨i, hi⟩
+      match σ.litValue lit with
+      | Sum.inr true => ⟨τ, true⟩
+      | Sum.inr false => go (i + 1) τ
+      | Sum.inl l =>
+        match τ.litValue? l with
+        | some true => ⟨τ, true⟩
+        | some false => go (i + 1) τ
+        | none => go (i + 1) (τ.setLit (-l))
+    else ⟨τ, false⟩
+  termination_by (F.rsize index) - i
+  go 0 τ
+
+def assumeWitness (σ : PS) (pivot : ILit) (A₁ : Array ILit) (A₂ : Array ILit) : PS :=
+  ((σ.reset.setLits A₁).setVars' A₂).setLit pivot
+
+def checkLine (F : RangeArray ILit) (τ : PPA) (σ : PS) (line : SRAdditionLine) : Except Bool (RangeArray ILit × PPA × PS) :=
+  let ⟨C, wL, wM, upHints, ratHintIndexes, ratHints, _, _⟩ := line
+  -- dbg_trace s!"{C}, {wL}, {wM}"
+  -- dbg_trace s!"{upHints}, {ratHintIndexes}, {ratHints}"
+  match assumeNegatedClauseFor τ.reset C (ratHints.size + 1) with
+  | error _ =>
+    -- dbg_trace s!"Assumed negation of clause had error"
+    error false
+  | ok τ =>
+    -- dbg_trace s!"Assumed negation of clause succeeded"
+    -- Evaluate the UP hints, with "# of RAT hints" as the offset
+    match applyUPHints F (ratHints.size + 1) τ upHints with
+    | error ⟨_, false⟩ =>
+      -- dbg_trace s!"Applying UP hints encountered an error"
+      error false
+    | error ⟨τ, true⟩ =>
+      -- dbg_trace s!"Applying UP hints found contradiction before RAT"
+      if C.size = 0 then error true    -- If the clause is empty, we have a successful contradiction proof
+      else ok ⟨F.add C, τ, σ⟩
+
+    | ok τ =>
+      -- If the clause is empty, we should have derived UP contradiction by now
+      if hC : 0 < C.size then
+        let pivot : ILit := wL.getD 0 (C.get ⟨0, hC⟩)
+        if pivot != C.get ⟨0, hC⟩ then error false else
+        let σ := assumeWitness σ pivot wL wM
+
+        -- Loop through each clause in the formula to check RAT conditions
+        -- The Bool is true if the check succeeds on all clauses, false otherwise
+        let Fsize := F.size
+        let rec loop (i cachedRatHintIndex bumpCounter : Nat) (τ : PPA) : PPA × Bool :=
+          if hi : i < Fsize then
+            if F.isDeleted i then loop (i + 1) cachedRatHintIndex bumpCounter τ
+            else
+              -- First, check how the ith clause is reduced by σ
+              match reduce σ F i with
+              | .satisfied => loop (i + 1) cachedRatHintIndex bumpCounter τ
+              | .notReduced => loop (i + 1) cachedRatHintIndex bumpCounter τ
+              | _ =>
+                -- dbg_trace s!"Clause index {i} is a RAT candidate"
+                if bumpCounter < ratHintIndexes.size then
+                  -- Find the corresponding RAT hint
+                  match findRATHintIndex cachedRatHintIndex i ratHintIndexes with
+                  | none => ⟨τ, false⟩
+                  | some ratIndex =>
+                    -- Assume the negation of the RAT clause
+                    match assumeRATClause F ⟨i, hi⟩ σ τ with
+                    | ⟨τ, true⟩ => loop (i + 1) (ratIndex + 1) (bumpCounter + 1) τ.bump
+                    | ⟨τ, false⟩ =>
+                      match applyUPHints F 0 τ (ratHints.get ⟨ratIndex, by sorry⟩) with
+                      | ok τ => ⟨τ, false⟩
+                      | error ⟨τ, false⟩ => ⟨τ, false⟩
+                      | error ⟨τ, true⟩ => loop (i + 1) (ratIndex + 1) (bumpCounter + 1) τ.bump
+                else ⟨τ, false⟩
+          else ⟨τ, true⟩
+        termination_by F.size - i
+
+        match loop 0 0 0 τ with
+        | ⟨_, false⟩ => error false
+        | ⟨τ, true⟩ => ok ⟨F.add C, τ, σ⟩
+
+      else error false
+
+end SR
+
+partial def main (args : List String) : IO Unit := do
+  let cnfFile := args[0]!
+  let lsrFile := args[1]!
+  let option : Nat := (args.getD 2 "0").toNat!
+  let contents ← IO.FS.withFile cnfFile .read (·.readToEnd)
+  let F : RangeArray ILit ← IO.ofExcept <| SRParser.parseFormula contents RangeArray.empty
+  IO.println s!"Formula has {F.size} clauses"
+
+  match option with
+  | 0 =>
+    let lsrContents : String ← IO.FS.withFile lsrFile .read (·.readToEnd)
+    let lines := lsrContents.splitOn "\n"
+      |>.filter (fun line => !line.startsWith "c" && line.any (!·.isWhitespace))
+
+    match lines.foldlM (init := (⟨F, PPA.new 100, PS.new 100⟩ : RangeArray ILit × PPA × PS))
+      (fun ⟨F, τ, σ⟩ line =>
+        match SRParser.parseLSRLine' F.size line with
+        | .error _ => throw false
+        | .ok ⟨_, Sum.inl l⟩ => SR.checkLine F τ σ l
+        | .ok (_, .inr l) =>
+          return ⟨l.clauses.foldl RangeArray.delete F, τ, σ⟩) with
+    | Except.ok _ =>
+      IO.println "c Proof failed to derive the empty clause, but is otherwise valid"
+      IO.println "s VALID"
+    | Except.error false => IO.println "c Proof failed"
+    | Except.error true => IO.println "s VERIFIED UNSAT"
+  | _ =>
+    let lsrContents : ByteArray ← IO.FS.withFile lsrFile .read (·.readBinToEnd)
+    let rec go (readPtr : Nat) (F : RangeArray ILit) (τ : PPA) (σ : PS) : IO Unit := do
+      if readPtr < lsrContents.size then
+        match SRParser.parseLSRLineBinary lsrContents readPtr with
+        | ok ⟨newPtr, lineId, .inl line⟩ =>
+          match SR.checkLine F τ σ line with
+          | Except.ok ⟨F, τ, σ⟩ => go newPtr F τ σ
+          | Except.error false => IO.println "c Proof failed"
+          | Except.error true => IO.println "s VERIFIED UNSAT"
+        | ok ⟨newPtr, lineId, .inr line⟩ =>
+          go newPtr (line.clauses.foldl RangeArray.delete F) τ σ
+        | error str => IO.println s!"c Error: {str}"
+      else
+        IO.println "c End of file"
+    go 0 F (PPA.new 100) (PS.new 100)
