Experiments/ProofChecking/SRCheckerEfficient.lean
@@ -1,0 +1,269 @@
+/-
+
+Theory and implementation for the SR proof system and a checker.
+
+Authors: Cayden Codel
+Carnegie Mellon University
+
+-/
+
+import Experiments.ProofChecking.PPA
+import Experiments.ProofChecking.PS
+import Experiments.ProofChecking.RangeArray
+
+import LeanSAT.Data.Cnf
+import LeanSAT.Data.ICnf
+import LeanSAT.Model.PropFun
+import LeanSAT.Model.Subst
+
+open LeanSAT LeanSAT.Model Nat
+open PPA PS LitVar ILit IVar LawfulLitVar PropFun
+open Except
+
+namespace PPA
+
+def unitPropFlat (τ : PPA) (F : RangeArray ILit) (i : Nat) : MUPResult :=
+  match F.foldlM_index (pevalUP τ) none i with
+  | ok none => .falsified
+  | ok (some lit) => .unit lit
+  | error .satisfied => .satisfied
+  | error .multipleUnassignedLiterals => .multipleUnassignedLiterals
+
+-- TODO: Some correctness theorem relating this to unitProp
+
+end PPA
+
+namespace PS
+
+def reduceFlat (σ : PS) (F : RangeArray ILit) (i : Nat) : ReductionResult :=
+  F.foldl_index (seval_fold_fn' σ) .notReduced i
+
+end PS
+
+namespace SR
+
+inductive UPResult
+  | checked : UPResult
+  | checkError : UPResult
+
+open UPResult
+
+structure SRLine where
+  clause : IClause
+  witness_lits : Array ILit
+  witness_maps : Array (IVar × ILit)
+  up_hints : Array Nat                -- Already 0-indexed clause IDs into the accumulated formula
+  rat_hints : Array (Nat × Array Nat) -- Already 0-indexed clause IDs into the accumulated formula
+
+structure SRState where
+  F : ICnf -- Accumulated formula
+  τ : PPA  -- Partial assignment, to store candidate and RAT negations
+  σ : PS   -- Substitution, for the witness
+
+-- Applies a single unit propagation step
+-- On success, we set the unit literal in τ with the offset
+-- On falsification of the clause, we error with .checked
+-- On satisfied clause or multiple unassigned literals, we error with checkError
+def applyUPHint (F : ICnf) (offset : Nat) (τ : PPA) (hint : Nat) : Except (PPA × UPResult) PPA :=
+  if h_hint : hint < F.size then
+    let C := F.get ⟨hint, h_hint⟩
+    match τ.unitProp C with
+    | .falsified => error ⟨τ, .checked⟩
+    | .satisfied =>
+      --dbg_trace s!"ERROR: UP found a satisfied clause"
+      error ⟨τ, .checkError⟩
+    | .multipleUnassignedLiterals =>
+      --dbg_trace s!"ERROR: UP found a non-unit clause"
+      error ⟨τ, .checkError⟩
+    | .unit l => ok (τ.setLitFor l offset)
+  else
+    --dbg_trace s!"ERROR: Hint out of bounds"
+    error ⟨τ, .checkError⟩
+
+def scanRATHints (clauseId : Nat) (ratHints : Array (Nat × Array Nat)) : Option (Fin ratHints.size) :=
+  match ratHints.foldlM (init := 0) (fun counter ⟨hint, _⟩ =>
+        if hint = clauseId then error counter
+        else ok (counter + 1)) with
+  | ok _ => none
+  | error index =>
+    if hi : index < ratHints.size then some ⟨index, hi⟩
+    else none
+
+-- Finds the RAT hint pair that matches the clauseId
+def findRATHintIndex (ratIndex clauseId : Nat) (ratHints : Array (Nat × Array Nat)) : Option (Fin ratHints.size) :=
+  -- If the RAT hints are sorted, then check the one under our "cached pointer" first
+  if h_index : ratIndex < ratHints.size then
+    let ⟨ratClauseIndex, _⟩ := ratHints.get ⟨ratIndex, h_index⟩
+    if ratClauseIndex = clauseId then some ⟨ratIndex, h_index⟩
+    else scanRATHints clauseId ratHints
+  else
+    scanRATHints clauseId ratHints
+
+-- Assuming that (C|σ) is reduced but not satisfied and that C is a RAT clause, sets τ ← τ ⊓ (C|σ)ᶜ
+def assumeRATClause (C : IClause) (σ : PS) (τ : PPA) : Except PPA PPA :=
+  C.foldlM (init := τ) (fun τ lit =>
+    match σ.litValue lit with
+    | Sum.inr true => error τ       -- (C|σ) is satisfied, so return early to report satisfied
+    | Sum.inr false => ok τ         -- Ignore the literal
+    | Sum.inl l =>
+      match τ.litValue? l with
+      | some true => error τ    -- (C|σ)|τ is satisfied, so return early to report satisfied
+      | some false => ok τ      -- Its negation is true in τ, so ignore the literal
+      | none => ok (τ.setLit (-l)))
+
+-- Set the witness substitution σ from the provided mapping, resetting σ first
+def assumeWitness (σ : PS) (pivot : ILit) (A₁ : Array ILit) (A₂ : Array (IVar × ILit)) : PS :=
+  ((σ.reset.setLits A₁).setVars A₂).setLit pivot
+
+structure FlatState where
+  formula : RangeArray ILit -- Accumulated formula
+  τ : PPA                   -- Partial assignment, to store candidate and RAT negations
+  σ : PS                    -- Substitution, for the witness
+
+-- Applies a single unit propagation step
+-- On success, we set the unit literal in τ with the offset
+-- On falsification of the clause, we error with .checked
+-- On satisfied clause or multiple unassigned literals, we error with checkError
+def applyUPHintFlat (F : RangeArray ILit) (offset : Nat) (τ : PPA) (hint : Nat) : Except (PPA × UPResult) PPA :=
+  if hint < F.size then
+    match τ.unitPropFlat F hint with
+    | .falsified => error ⟨τ, .checked⟩
+    | .satisfied =>
+      -- dbg_trace s!"ERROR: UP found a satisfied clause"
+      error ⟨τ, .checkError⟩
+    | .multipleUnassignedLiterals =>
+      -- dbg_trace s!"ERROR: UP found a non-unit clause"
+      error ⟨τ, .checkError⟩
+    | .unit l =>
+      -- dbg_trace s!"    Hint {hint} makes clause unit on literal {l}"
+      ok (τ.setLitFor l offset)
+  else
+    -- dbg_trace s!"ERROR: Hint out of bounds"
+    error ⟨τ, .checkError⟩
+
+-- Assuming that (C|σ) is reduced but not satisfied and that C is a RAT clause, sets τ ← τ ⊓ (C|σ)ᶜ
+def assumeRATClauseFlat (F : RangeArray ILit) (i : Nat) (σ : PS) (τ : PPA) : Except PPA PPA :=
+  F.foldlM_index (i := i) (init := τ) (fun τ lit =>
+    match σ.litValue lit with
+    | Sum.inr true => error τ       -- (C|σ) is satisfied, so return early to report satisfied
+    | Sum.inr false => ok τ         -- Ignore the literal
+    | Sum.inl l =>
+      match τ.litValue? l with
+      | some true => error τ    -- (C|σ)|τ is satisfied, so return early to report satisfied
+      | some false => ok τ      -- Its negation is true in τ, so ignore the literal
+      | none => ok (τ.setLit (-l)))
+
+-- Check each clause in the formula.
+-- C is the current clause in the formula to be checked for the RAT property under σ and τ
+-- If C is reduced by σ, then it is RAT. Find a RAT hint and uses the RAT UP hints to derive contradiction.
+def checkClauseFlat (F : RangeArray ILit) (σ : PS) (ratHints : Array (Nat × Array Nat))
+    (p : PPA × Nat × Nat) (i : Nat) : Except Unit (PPA × Nat × Nat) :=
+  let ⟨τ, ratIndex, bumpCounter⟩ := p
+  match σ.reduceFlat F i with
+  | .satisfied => ok (τ, ratIndex, bumpCounter)
+  | .notReduced => ok (τ, ratIndex, bumpCounter)
+  | _ =>
+    -- dbg_trace s!"     Clause {i} is reduced, checking for RAT"
+    -- We expect a RAT clause. Check if we have bumps left
+    if bumpCounter < ratHints.size then
+      -- Curiously, if the clause is completely falsified, we can still succeed
+      -- on the check (which sr-check does not allow). This is because a UP
+      -- derivation on a completely falsified clause is a global UP derivation,
+      -- and so the certificate can be reduced quite a bit.
+
+      -- Find a RAT hint matching the clause (add one to the current index, due to 1-indexing)
+      -- We hope that the hints are sorted, but they don't have to be
+      match findRATHintIndex ratIndex i ratHints with
+      | none =>
+        -- dbg_trace s!"Clause {i} found to be missing a RAT hint"
+        error ()
+      | some rI =>
+        let ⟨_, hints⟩ := ratHints.get rI
+        match assumeRATClauseFlat F i σ τ with
+        -- If the clause is satisfied under σ and τ, then we move to the next iteration
+        | error τ => ok (τ.bump, rI.val + 1, bumpCounter + 1)
+
+        -- Otherwise, we have assumed the negation of the RAT clause
+        -- Now check for UP derivation through its hints
+        | ok τ =>
+          match hints.foldlM (init := τ) (applyUPHintFlat F 0) with
+          | error (τ, .checked) => ok (τ.bump, rI.val + 1, bumpCounter + 1)
+          | error (_, .checkError) =>
+            -- dbg_trace s!"ERROR: UP failed"
+            error ()
+          | ok _ =>
+            -- dbg_trace s!"ERROR: UP succeeded, but didn't lead to contradiction"
+            error ()
+    -- We error if the bumpCounter equals the number of RAT hints, since that
+    -- means we bumped the assignment too many times, clearing out the
+    -- assumption of the candidate clause
+    else
+      -- dbg_trace s!"ERROR: Bump counter exceeded number of RAT hints"
+      error ()
+
+def checkLineFlat (S : FlatState) (line : SRLine) : Except Bool FlatState :=
+  -- dbg_trace s!"About to check line with clause {line.clause}"
+  let ⟨F, τ, σ⟩ := S
+  let ⟨C, w_tf, w_maps, UPhints, RAThints⟩ := line
+
+  -- Assumes the negation of the candidate clause, with "# of RAT hints" offset
+  match assumeNegatedClauseFor τ.reset C (RAThints.size + 1) with
+  | error _ =>
+    -- dbg_trace s!"ERROR: Assumption of clause failed"
+    error false
+  | ok τ =>
+
+  -- dbg_trace s!"Assumed negation of {C} with {RAThints.size + 1} offset"
+
+  -- Evaluate the UP hints, with "# of RAT hints" offset
+  -- We add one more than normal to help with proving
+  match UPhints.foldlM (init := τ) (applyUPHintFlat F (RAThints.size + 1)) with
+  -- The clause led to contradiction via unit propagation
+  | error ⟨τ, .checked⟩ =>
+    if C = #[] then error true       -- If the clause is empty, we have a successful proof
+    else ok ⟨F.add C, τ, σ⟩ -- The clause is redundant, so add it to the formula
+
+  -- Unit propagation failed due to multiple unassigned literals, satisfied clause, or out-of-bounds
+  | error ⟨_, _⟩ =>
+    -- dbg_trace s!"ERROR: UP failed"
+    error false
+
+  -- Unit propagation worked but didn't lead to contradiction, so continue to RAT checking
+  | ok τ =>
+
+    -- dbg_trace s!"  UP succeeded, checking for RAT"
+
+    -- If the clause is empty, then we should have derived UP contradiction by now
+    if hCw : 0 < C.size ∧ 0 < w_tf.size then
+      if C.get ⟨0, hCw.1⟩ ≠ w_tf.get ⟨0, hCw.2⟩ then
+        -- dbg_trace s!"Pivot doesn't agree with 0th literal"
+        error false
+      else
+
+      -- Assume the witness, under substitution (the function call resets σ)
+      let σ := assumeWitness σ (C.get ⟨0, hCw.1⟩) w_tf w_maps
+      -- dbg_trace s!"{σ}"
+
+      -- Go through each clause in the formula to check RAT
+      let Fsize := F.size
+      let rec loop (i : Nat) (p : PPA × Nat × Nat) := do
+        if i < Fsize then
+          loop (i + 1) (← checkClauseFlat F σ RAThints p i)
+        else
+          pure p
+        termination_by Fsize - i
+
+      --match F.foldlM_over_indexes (init := (⟨τ, 0, 0⟩ : PPA × Nat × Nat)) (checkClauseFlat F σ RAThints) with
+      match loop 0 ⟨τ, 0, 0⟩ with
+      | error () =>
+        -- dbg_trace s!"ERROR: RAT check failed"
+        error false
+      | ok (τ, _) =>
+        -- dbg_trace s!"RAT check succeeded, adding clause {C}"
+        ok ⟨F.add C, τ, σ⟩ -- The RAT hint checked, so we continue
+
+    else
+      -- dbg_trace s!"ERROR: Either the clause or the true/false mappings are empty"
+      error false
+
+end SR
