Experiments/ProofChecking/SRParserBasic.lean
@@ -1,0 +1,430 @@
+/-
+
+A basic SR parser for general formulas.
+
+Author: Cayden Codel
+Carnegie Mellon University
+
+-/
+
+import LeanSAT.Solver.Dimacs
+import Experiments.ProofChecking.RangeArray
+
+open Std
+open LeanSAT.Solver.Dimacs
+open LeanSAT LeanSAT.Model ILit Except
+
+namespace SR
+
+structure SRAdditionLine where
+  witnessLits : Array ILit
+  witnessMaps : Array ILit     -- Maps literals to literals
+  upHints : Array Nat          -- Already 0-indexed clause IDs into the accumulated formula
+  ratHintIndexes : Array Nat   -- Already 0-indexed
+  ratHints : Array (Array Nat) -- Already 0-indexed
+  ratSizesEq : ratHintIndexes.size = ratHints.size
+  witnessMapsMod : witnessMaps.size % 2 = 0
+  -- CC: Technically, ratHints can be a RangeArray. Try later
+
+def SRAdditionLine.new : SRAdditionLine := ⟨
+  Array.mkEmpty 100,
+  Array.mkEmpty 100,
+  Array.mkEmpty 100,
+  Array.mkEmpty 100,
+  Array.mkEmpty 100,
+  by simp, by simp⟩
+
+instance : Inhabited SRAdditionLine := ⟨{
+  witnessLits := #[],
+  witnessMaps := #[],
+  upHints := #[],
+  ratHintIndexes := #[],
+  ratHints := #[],
+  ratSizesEq := by simp,
+  witnessMapsMod := by simp
+}⟩
+
+structure SRDeletionLine where
+  clauses : Array Nat
+deriving Inhabited
+
+end SR
+
+namespace SRParser
+
+protected class Formula (F : Type _) where
+  empty : F
+  addLiteral : F → ILit → F
+  commitClause : F → F
+  size : F → Nat
+
+instance : SRParser.Formula (RangeArray ILit) where
+  empty := (RangeArray.empty : RangeArray ILit)
+  addLiteral := RangeArray.addElement
+  commitClause := RangeArray.commit
+  size := RangeArray.size
+
+instance : SRParser.Formula (ICnf × IClause) where
+  empty := (#[], #[])
+  addLiteral := (fun ⟨F, C⟩ l => ⟨F, C.push l⟩)
+  commitClause := (fun ⟨F, C⟩ => (F.push C, #[]))
+  size := (fun ⟨F, _⟩ => F.size)
+
+variable {CNF : Type _} [SRParser.Formula CNF]
+
+-- Parses a single literal from a string.
+-- CC: The double Except monad is used to stop folding across a list/array of atom strings
+--     in case a 0 is encountered, since DIMACS doesn't require a clause to fit on a line.
+@[inline, specialize]
+def parseLit (maxVar : Nat) (F : CNF) (s : String) : Except (Except String CNF) CNF := do
+  match s.toInt? with
+  | none => throw (throw s!"Literal is not a number: {s}")
+  | some n =>
+    if hn : n = 0 then
+      throw (return F)
+    else
+      if n.natAbs > maxVar then
+        throw (throw s!"Literal {n} is greater than the maximum variable {maxVar}")
+      else
+        return Formula.addLiteral F ⟨n, hn⟩
+
+@[specialize]
+def parseClause (maxVar : Nat) (F : CNF) (s : String) : Except String CNF :=
+  match s.splitOn " " |>.foldlM (parseLit maxVar) F with
+  | ok _ => throw "Zero not encountered on this line"
+  | error e => return Formula.commitClause (← e)
+
+-- Parses the CNF given a string and an empty formula to read the clauses into
+def parseFormula (s : String) (F : CNF) : Except String CNF := do
+  match s.splitOn "\n" |>.filter (fun line => !line.startsWith "c" && line.any (!·.isWhitespace)) with
+  | [] => throw "All lines are empty or comments"
+  | (pLine :: clauseLines) =>
+    let (nvars, ncls) ← parseHeader pLine
+    let F ← clauseLines.foldlM (parseClause nvars) F
+    if SRParser.Formula.size F != ncls then
+      throw s!"Expected {ncls} clauses, but found {Formula.size F}"
+    else
+      return F
+
+inductive SRParsingMode
+| clause
+| witnessLits
+| witnessMappedReady
+| witnessMappedHalfway : IVar → SRParsingMode
+| upHints
+| ratHints : Nat → Array Nat → SRParsingMode
+| lineDone
+| err : String → SRParsingMode
+deriving BEq, Inhabited
+
+open SR SRParsingMode
+
+@[inline]
+def processSRAtom (atom : Int) (pivot : Option ILit)
+    (line : SRAdditionLine) (F : CNF) (mode : SRParsingMode) : SRAdditionLine × CNF × SRParsingMode :=
+  if h_atom : atom = 0 then
+    match mode with
+    | .clause =>
+      -- We don't have a witness, so we insert the pivot into the witness and continue, if the clause isn't empty
+      match pivot with
+      | none => ⟨line, F, .upHints⟩
+      | some pivot => ⟨{ line with witnessLits := line.witnessLits.push pivot }, F, .upHints⟩
+    | .witnessLits => ⟨line, F, .upHints⟩
+    | .witnessMappedReady => ⟨line, F, .upHints⟩
+    | .witnessMappedHalfway _ => ⟨line, F, .err "Only got half a substitution mapping when ending a witness"⟩
+    | .upHints => ⟨line, F, .lineDone⟩
+    | .ratHints index hints => ⟨{ line with
+        ratHintIndexes := line.ratHintIndexes.push index,
+        ratHints := line.ratHints.push hints,
+        ratSizesEq := by simp [line.ratSizesEq] }, F, .lineDone⟩
+    | .lineDone => ⟨line, F, .err "Addition line continued after last ending 0"⟩
+    | .err str => ⟨line, F, .err str⟩
+  else
+    match mode with
+    | .clause =>
+      match pivot with
+      | none => ⟨line, F, .err "No pivot provided for the clause"⟩
+      | some pivot =>
+        if atom = pivot.val then
+          -- Seeing the pivot again means we're parsing a witness
+          ⟨{ line with witnessLits := line.witnessLits.push ⟨atom, h_atom⟩ }, F, .witnessLits⟩
+        else
+          -- It's not the pivot (and it's not 0), so add it to the clause
+          ⟨line, SRParser.Formula.addLiteral F ⟨atom, h_atom⟩, .clause⟩
+    | .witnessLits =>
+      match pivot with
+      | none => ⟨line, F, .err "No pivot provided for the witness"⟩
+      | some pivot =>
+        if atom = pivot.val then
+          -- Seeing the pivot again means we're parsing the substitution mappings
+          ⟨line, F, .witnessMappedReady⟩
+        else
+          ⟨{ line with witnessLits := line.witnessLits.push ⟨atom, h_atom⟩ }, F, .witnessLits⟩
+    | .witnessMappedReady =>
+      match pivot with
+      | none => ⟨line, F, .err "No pivot provided for the witness"⟩
+      | some pivot =>
+        if atom = pivot.val then
+          ⟨line, F, .err "Saw pivot again in substitution mapping"⟩
+        else
+          if atom < 0 then
+            ⟨line, F, .err "First of a substitution mapping must be positive"⟩
+          else
+            ⟨line, F, .witnessMappedHalfway ⟨atom.natAbs, Int.natAbs_pos.mpr h_atom⟩⟩
+    | .witnessMappedHalfway v =>
+      ⟨{line with
+        witnessMaps := line.witnessMaps.push v |>.push ⟨atom, h_atom⟩,
+        witnessMapsMod := by simp [add_assoc, Nat.add_mod_right, line.witnessMapsMod] }, F, .witnessMappedReady⟩
+    | .upHints =>
+      if atom < 0 then
+        match pivot with
+        | none => ⟨line, F, .err "Can't have RAT hints for empty clauses"⟩
+        | _ =>
+          -- This is our first RAT hint - start building it
+          ⟨line, F, .ratHints (atom.natAbs - 1) #[]⟩
+      else
+        ⟨{ line with upHints := line.upHints.push (atom.natAbs - 1) }, F, .upHints⟩
+    | .ratHints index hints =>
+      if atom < 0 then
+        -- This is a new RAT hint - add the old one
+        ⟨{ line with
+          ratHintIndexes := line.ratHintIndexes.push index,
+          ratHints := line.ratHints.push hints,
+          ratSizesEq := by simp [line.ratSizesEq] }, F, .ratHints (atom.natAbs - 1) #[]⟩
+      else
+        ⟨line, F, .ratHints index (hints.push (atom.natAbs - 1))⟩
+    | .lineDone => ⟨line, F, .err "Addition line continued after last ending 0"⟩
+    | .err str => ⟨line, F, .err str⟩
+
+def parseSRAtom (pivot : Option ILit) (line : SRAdditionLine) (F : CNF) (mode : SRParsingMode) (s : String) : SRAdditionLine × CNF × SRParsingMode :=
+  -- No matter what, the string should be a number, so parse it as an int
+  match s.toInt? with
+  | none => ⟨line, F, .err s!"Atom {s} didn't parse to a number"⟩
+  | some n => processSRAtom n pivot line F mode
+
+def parseLSRLine (F : CNF) (maxId : Nat) (s : String) : Except String (Nat × CNF × (SRAdditionLine ⊕ SRDeletionLine)) :=
+  match s.splitOn " " with
+  | [] => throw "Empty line"
+  | [_] => throw s!"Single atom line: {s}, with id {maxId}"
+  | (id :: hd :: tls) =>
+    match hd with
+    | "d" =>
+      -- Check to make sure the maxId is (non-strictly) monotonically increasing
+      match id.toNat? with
+      | none => throw "Line ID is not a number"
+      | some id =>
+        if id < maxId then
+          throw "Deletion line id is not increasing"
+        else
+          match tls.foldlM (fun arr str =>
+            match str.toNat? with
+            | none => throw (throw s!"{str} was not a number")
+            | some 0 => throw (return arr)
+            | some (n + 1) => return arr.push n) #[] with
+          | ok _ => throw "Zero not found on deletion line"
+          | error e => return ⟨max id maxId, F, .inr (SRDeletionLine.mk (← e))⟩
+    | _ =>
+      -- We have an addition line, so the maxId should strictly increase
+      match id.toNat? with
+      | none => throw "Line ID is not a number"
+      | some id =>
+        if id ≤ maxId then
+          throw s!"Addition line id is not increasing: parsed {id}, max {maxId}"
+        else
+          match hd.toInt? with
+          | none => throw "Pivot is not a number"
+          | some n =>
+            let line := SRAdditionLine.new
+            let res :=
+              if hn : n = 0 then
+                tls.foldlM (init := (⟨line, F, .upHints⟩ : SRAdditionLine × CNF × SRParsingMode))
+                  (fun ⟨line, F, mode⟩ s => match mode with
+                    | .err s => error s
+                    | m => ok <| parseSRAtom none line F m s)
+              else
+                tls.foldlM (init := ⟨line, SRParser.Formula.addLiteral F ⟨n, hn⟩, .clause⟩)
+                  (fun ⟨line, F, mode⟩ s => match mode with
+                    | .err s => error s
+                    | m => ok <| parseSRAtom (some ⟨n, hn⟩) line F m s)
+            match res with
+            | error str => throw str
+            | ok ⟨line, F, mode⟩ =>
+              if mode != .lineDone then
+                throw "Addition line didn't end with 0"
+              else
+                return ⟨id, F, .inl line⟩
+
+-- CC: An attempt to get parsing faster, given that the Except monad can be expensive
+def parseLSRLine'_aux (pivot : Option ILit) (line : SRAdditionLine) (F : CNF) (mode : SRParsingMode) : List String → (SRAdditionLine × CNF × SRParsingMode)
+  | [] => (line, F, mode)
+  | atom :: atoms =>
+  -- No matter what, the string should be a number, so parse it as an int
+  match atom.toInt? with
+  | none => ⟨line, F, .err s!"Atom {atom} didn't parse to a number"⟩
+  | some n =>
+    match processSRAtom n pivot line F mode with
+    | ⟨line, F, .err str⟩ => ⟨line, F, .err str⟩
+    | ⟨line, F, mode⟩ => parseLSRLine'_aux pivot line F mode atoms
+
+def parseLSRLine' (F : CNF) (maxId : Nat) (s : String) : Except String (Nat × CNF × (SRAdditionLine ⊕ SRDeletionLine)) :=
+  match s.splitOn " " with
+  | [] => throw "Empty line"
+  | [_] => throw s!"Single atom line: {s}, with id {maxId}"
+  | (id :: hd :: tls) =>
+    match hd with
+    | "d" =>
+      -- Check to make sure the maxId is (non-strictly) monotonically increasing
+      match id.toNat? with
+      | none => throw "Line ID is not a number"
+      | some id =>
+        if id < maxId then
+          throw "Deletion line id is not increasing"
+        else
+          match tls.foldlM (fun arr str =>
+            match str.toNat? with
+            | none => throw (throw s!"{str} was not a number")
+            | some 0 => throw (return arr)
+            | some (n + 1) => return arr.push n) #[] with
+          | ok _ => throw "Zero not found on deletion line"
+          | error e => return ⟨max id maxId, F, .inr (SRDeletionLine.mk (← e))⟩
+    | _ =>
+      -- We have an addition line, so the maxId should strictly increase
+      match id.toNat? with
+      | none => throw "Line ID is not a number"
+      | some id =>
+        if id ≤ maxId then
+          throw s!"Addition line id is not increasing: parsed {id}, max {maxId}"
+        else
+          match hd.toInt? with
+          | none => throw "Pivot is not a number"
+          | some n =>
+            let line := SRAdditionLine.new
+            let res :=
+              if hn : n = 0 then
+                parseLSRLine'_aux none line F .upHints tls
+              else
+                parseLSRLine'_aux (some ⟨n, hn⟩) line (SRParser.Formula.addLiteral F ⟨n, hn⟩) .clause tls
+            match res with
+            | ⟨_, _, .err str⟩ => throw str
+            | ⟨line, F, mode⟩ =>
+              if mode != .lineDone then
+                throw "Addition line didn't end with 0"
+              else
+                return ⟨id, F, .inl line⟩
+
+--------------------------------------------------------------------------------
+
+def undoBinaryMapping (x : UInt64) : Int :=
+  if x &&& 1 = 1 then
+    ((((x >>> 1).toNat) : Int) * -1)
+  else
+    (((x >>> 1).toNat) : Int)
+
+/-
+def readBinaryToken (A : ByteArray) (index : Nat) : Int × { i : Nat // i > index } :=
+  let rec go (i : Nat) (acc : UInt64) (shift : UInt64) : Int × { idx : Nat // idx > i } :=
+    if hi : i < A.size then
+      let atom : UInt8 := A.get ⟨i, hi⟩
+      let acc' : UInt64 := acc ||| ((atom &&& 127).toUInt64 <<< shift)
+      if atom &&& 128 != 0 then
+        match go (i + 1) acc' (shift + 7) with
+        | ⟨a, ⟨b, hb⟩⟩ => ⟨a, ⟨b, Nat.le_of_succ_le hb⟩⟩
+      else
+        ⟨undoBinaryMapping acc', ⟨A.size, hi⟩⟩
+    else
+      ⟨undoBinaryMapping acc, ⟨i + 1, Nat.lt_succ_self _⟩⟩
+  termination_by A.size - i
+  go index 0 0
+-/
+
+-- Int is result, Nat is cached index into A
+partial def readBinaryToken (A : ByteArray) (index : Nat) : Int × Nat :=
+  let rec go (i : Nat) (acc : UInt64) (shift : UInt64) : Int × Nat :=
+    if hi : i < A.size then
+      let atom : UInt8 := A.get ⟨i, hi⟩
+      let acc' : UInt64 := acc ||| ((atom &&& 127).toUInt64 <<< shift)
+      if atom &&& 128 != 0 then
+        go (i + 1) acc' (shift + 7)
+      else
+        ⟨undoBinaryMapping acc', i + 1⟩
+    else
+      ⟨undoBinaryMapping acc, A.size⟩
+  let ⟨res, idx⟩ := go index 0 0
+  -- dbg_trace s!"Pointer at index {index} moved to {idx}, parsed {res}"
+  ⟨res, idx⟩
+
+-- Bool: found a 0
+-- Nat: updated index
+partial def parseLSRDeletionLineBinary (A : ByteArray) (index : Nat) : Bool × Nat × SRDeletionLine :=
+  let rec go (i : Nat) (acc : Array Nat) : Bool × Nat × SRDeletionLine :=
+    if i < A.size then
+      let (x, j) := readBinaryToken A i
+      if x = 0 then
+        ⟨true, j, SRDeletionLine.mk acc⟩
+      else
+        go j (acc.push (x.natAbs - 1))
+    else
+      ⟨false, A.size, SRDeletionLine.mk acc⟩
+  go index #[]
+
+instance [Inhabited CNF] : Inhabited (Nat × SRAdditionLine × CNF × SRParsingMode) := by infer_instance
+
+/-
+partial def parseLSRAdditionLineBinary [Inhabited CNF] (F : CNF) (A : ByteArray)
+    (index : Nat) (pivot : Option ILit) : Nat × SRAdditionLine × CNF × SRParsingMode :=
+  let rec go (i : Nat) (line : SRAdditionLine) (F : CNF) (mode : SRParsingMode) : Nat × SRAdditionLine × CNF × SRParsingMode :=
+    if i < A.size then
+      let (n, j) := readBinaryToken A i
+      match processSRAtom n pivot line F mode with
+      | ⟨line, F, .err str⟩ => ⟨j, line, F, .err str⟩
+      | ⟨line, F, .lineDone⟩ => ⟨j, line, F, .lineDone⟩
+      | ⟨line, F, mode⟩ => go j line F mode
+    else
+      ⟨A.size, line, F, mode⟩
+
+  let newLine := SRAdditionLine.new
+  match pivot with
+  | none => go index newLine F .upHints
+  | some p => go index newLine (SRParser.Formula.addLiteral F p) .clause -/
+
+
+-- First nat is cached index into arr, second is ID of new clause to add
+/-
+partial def parseLSRLineBinary (A : ByteArray)
+    (index : Nat) : Except String (Nat × Nat × (SRAdditionLine ⊕ SRDeletionLine)) :=
+  if hi : index + 1 < A.size then
+    -- Check if we have an addition line or a deletion line
+    let lineStart : UInt8 := A.get ⟨index, Nat.lt_of_succ_lt hi⟩
+    let ⟨lineId, index⟩ := readBinaryToken A (index + 1)
+    if lineId < 0 then error "Negative line ID" else
+
+    -- Addition line
+    if lineStart = 1 then
+      -- Check if we have a pivot
+      if index < A.size then
+        let ⟨pivot, index⟩ := readBinaryToken A index
+        let res :=
+          if hp : pivot = 0 then
+            parseLSRAdditionLineBinary A index none
+          else
+            parseLSRAdditionLineBinary A index (some ⟨pivot, hp⟩)
+        match res with
+        | ⟨_, _, .err str⟩ => throw str
+        | ⟨index, line, mode⟩ =>
+          if mode != .lineDone then
+            error "Addition line didn't end with 0"
+          else
+            ok (index, lineId.natAbs, .inl line)
+      else
+        error "Line ended early"
+    else if lineStart = 2 then
+      match parseLSRDeletionLineBinary A index with
+      | ⟨true, index, line⟩ => ok (index, lineId.natAbs, .inr line)
+      | ⟨false, _, _⟩ => error "Deletion line didn't end with 0"
+    else
+      error "Start of line wasn't addition (1) or deletion (2)"
+
+  else
+    error "No more string!" -/
+
+end SRParser
