Experiments/ProofChecking/StatefulSR.lean
@@ -1,0 +1,320 @@
+/-
+
+SR checking with state monads.
+
+Cayden Codel
+-/
+
+import LeanSAT.Data.Cnf
+import LeanSAT.Data.Literal
+import LeanSAT.Data.ICnf
+
+import LeanSAT.Model.PropFun
+
+import Experiments.ProofChecking.PPA
+import Experiments.ProofChecking.PS
+import Experiments.ProofChecking.RangeArray
+
+open LeanSAT LeanSAT.Model PropFun
+
+namespace SR
+/-
+@[inline, specialize]
+def foldlM_index {β : Type v} {m : Type v → Type w} [Monad m] (f : β → α → m β)
+    (init : β) (A : RangeArray α) (i : Nat) : m β :=
+  A.data.foldlM f init (A.index i) (A.index i + A.rsize i)
+-/
+-- A typeclass for Formulas. Supports the basic operations needed for SR checking.
+@[specialize]
+class Formula (F : Type u) where
+  size : F → Nat
+  empty : F
+  addClause : F → IClause → F
+  deleteClause : F → Nat → F
+  isDeleted : F → Nat → Bool
+  foldMOnClause : F → Nat →
+    {β : Type v} → {m : Type v → Type w} → [Monad m] →
+    (f : β → ILit → m β) → (init : β) → m β
+  -- Technically, `toPropFun` can be defined in terms of foldMOnClause
+  --toPropFun : F → PropFun IVar
+
+open Formula in
+class LawfulFormula (F : Type u) [Formula F] where
+  size_empty : size (empty : F) = 0
+  size_addClause (f : F) (c : IClause) : size (addClause f c) = size f + 1
+  size_deleteClause (f : F) (i : Nat) : size (deleteClause f i) = size f
+  /-- All clauses out-of-bounds are deleted. -/
+  isDeleted_ge_size (f : F) (i : Nat) : i ≥ size f → isDeleted f i = false
+  /-- If we delete a clause, it should actually be marked as deleted. -/
+  isDeleted_deleteClause (f : F) (i j : Nat) : isDeleted (deleteClause f i) j =
+    if i = j then true else isDeleted f j
+  /-- Added clauses are, by default, not deleted. -/
+  isDeleted_addClause (f : F) (c : IClause) (i : Nat) : isDeleted (addClause f c) (size f) = false
+  /-- Folding across a just-deleted clause should give back init. -/
+  foldlMOnClause_deleteClause (f : F) (i : Nat) {β : Type v} {m : Type v → Type w} [Monad m]
+    (g : β → ILit → m β) (init : β) : foldMOnClause (deleteClause f i) i g init = pure init
+  /-- If we fold after adding, it's the same as folding across either a clause in the formula,
+      or the clause we just added. -/
+  foldlMOnClause_addClause (f : F) (c : IClause) (i : Nat) {β : Type v} {m : Type v → Type w} [Monad m]
+    (g : β → ILit → m β) (init : β) : foldMOnClause (addClause f c) i g init =
+      if i = size f then c.foldlM g init else foldMOnClause f i g init
+
+structure SRState (CNF : Type _) [Formula CNF] where
+  F : CNF
+  τ : PPA
+  σ : PS
+
+structure SRLine where
+  clause : IClause
+  witness_lits : Array ILit
+  witness_maps : Array (IVar × ILit)
+  up_hints : Array Nat                -- Already 0-indexed clause IDs into the accumulated formula
+  rat_hints : Array (Nat × Array Nat) -- Already 0-indexed clause IDs into the accumulated formula
+
+abbrev ESt (CNF : Type _) [Formula CNF] := fun ε α => EStateM ε (SRState CNF) α
+abbrev St (CNF : Type _) [Formula CNF] := fun α => StateM (SRState CNF) α
+
+open Nat Formula PPA PS EStateM
+
+variable {CNF : Type _} [Formula CNF]
+
+namespace ESt
+
+variable {ε : Type _} {m : Type u → Type v} [Monad m] {β : Type u}
+
+@[always_inline, inline]
+protected def size : ESt CNF ε Nat :=
+  modifyGet (fun S => (Formula.size S.F, S))
+
+@[always_inline, inline]
+protected def foldMOnClause (i : Nat) (f : β → ILit → m β) (init : β) : ESt CNF ε (m β) :=
+  modifyGet (fun S => ((Formula.foldMOnClause S.F i f init), S))
+
+-- TODO: Better way to write this?
+#check EStateM.modifyGet
+
+@[always_inline, inline]
+protected def setLitFor (l : ILit) (offset : Nat) : ESt CNF ε Unit :=
+  modifyGet (fun S => ⟨(), { S with τ := S.τ.setLitFor l offset }⟩)
+
+@[always_inline, inline]
+protected def addClause (C : IClause) : ESt CNF ε Unit :=
+  modifyGet (fun S => ⟨(), { S with F := Formula.addClause S.F C }⟩)
+
+end ESt
+
+namespace St
+
+variable {m : Type u → Type v} [Monad m] {β : Type u}
+
+@[always_inline, inline]
+protected def size : St CNF Nat :=
+  modifyGet (fun S => (Formula.size S.F, S))
+
+@[always_inline, inline]
+protected def foldMOnClause (i : Nat) (f : β → ILit → m β) (init : β) : St CNF (m β) :=
+  modifyGet (fun S => ((Formula.foldMOnClause S.F i f init), S))
+
+@[always_inline, inline]
+protected def setLitFor (l : ILit) (offset : Nat) : St CNF Unit :=
+  modifyGet (fun S => ⟨(), { S with τ := S.τ.setLitFor l offset }⟩)
+
+@[always_inline, inline]
+protected def addClause (C : IClause) : St CNF Unit :=
+  modifyGet (fun S => ⟨(), { S with F := Formula.addClause S.F C }⟩)
+
+-- Basically lifts StateM to EStateM
+@[always_inline, inline]
+protected def ebind (x : StateT σ Id α) (f : α → EStateM ε σ β) : EStateM ε σ β :=
+  fun s => let (a, s) := x s; f a s
+
+end St
+
+-- TODO: Make this be a function in PPA for general UPBox
+-- TODO: Determine if this is faster than `do (← get).F.size, etc`
+open MUPResult in
+def SRfoldUP (i : Nat) : St CNF MUPResult := fun ⟨F, τ, σ⟩ =>
+  ⟨unitPropRes <| Formula.foldMOnClause F i (pevalUP τ) none, ⟨F, τ, σ⟩⟩
+
+open ReductionResult in
+def SRreduce (i : Nat) : St CNF ReductionResult := fun ⟨F, τ, σ⟩ =>
+  (reduceRes <| Formula.foldMOnClause F i (seval σ) false, ⟨F, τ, σ⟩)
+
+-- Applies a single unit propagation step
+-- On success, we set the unit literal in τ with the offset
+-- On falsification of the clause, we error with true (.checked)
+-- On satisfied clause or multiple unassigned literals, we error with false (.checkError)
+def applyUPHint (offset hint : Nat) : ESt CNF Bool Unit := fun ⟨F, τ, σ⟩ =>
+  if hint < size F then
+    match SRfoldUP hint ⟨F, τ, σ⟩ with
+    | ⟨.falsified, ⟨F, τ, σ⟩⟩ =>
+      EStateM.throw true ⟨F, τ, σ⟩
+    | ⟨.satisfied, ⟨F, τ, σ⟩⟩ =>
+      -- dbg_trace s!"ERROR: UP found a satisfied clause"
+      EStateM.throw false ⟨F, τ, σ⟩
+    | ⟨.multipleUnassignedLiterals, ⟨F, τ, σ⟩⟩ =>
+      -- dbg_trace s!"ERROR: UP found a non-unit clause"
+      EStateM.throw false ⟨F, τ, σ⟩
+    | ⟨.unit l, ⟨F, τ, σ⟩⟩ =>
+      Result.ok () { F, τ := τ.setLitFor l offset, σ }
+  else
+    EStateM.throw false ⟨F, τ, σ⟩
+
+def scanRATHints (clauseId : Nat) (ratHints : Array (Nat × Array Nat)) : Option (Fin ratHints.size) :=
+  match ratHints.foldlM (init := 0) (fun counter ⟨hint, _⟩ =>
+        if hint = clauseId then Except.error counter
+        else Except.ok (counter + 1)) with
+  | Except.ok _ => none
+  | Except.error index =>
+    if hi : index < ratHints.size then some ⟨index, hi⟩
+    else none
+
+-- Finds the RAT hint pair that matches the clauseId
+def findRATHintIndex (ratIndex clauseId : Nat) (ratHints : Array (Nat × Array Nat)) : Option (Fin ratHints.size) :=
+  -- If the RAT hints are sorted, then check the one under our "cached pointer" first
+  if h_index : ratIndex < ratHints.size then
+    let ⟨ratClauseIndex, _⟩ := ratHints.get ⟨ratIndex, h_index⟩
+    if ratClauseIndex = clauseId then some ⟨ratIndex, h_index⟩
+    else scanRATHints clauseId ratHints
+  else
+    scanRATHints clauseId ratHints
+
+-- `i` is the index into the formula
+-- Assuming that (C|σ) is reduced but not satisfied and that C is a RAT clause, sets τ ← τ ⊓ (C|σ)ᶜ
+def assumeRATClause (i : Nat) : ESt CNF Unit Unit := fun ⟨F, τ, σ⟩ =>
+  if i < size F then
+    match Formula.foldMOnClause F i (init := τ) (fun τ lit =>
+      match σ.litValue lit with
+      | .tr => Except.error τ       -- (C|σ) is satisfied, so return early to report satisfied
+      | .fls => Except.ok τ         -- Ignore the literal
+      | .lit l =>
+        match τ.litValue? l with
+        | some true => Except.error τ    -- (C|σ)|τ is satisfied, so return early to report satisfied
+        | some false => Except.ok τ      -- Its negation is true in τ, so ignore the literal
+        | none => Except.ok (τ.setLit (-l))) with
+    | Except.ok τ => Result.ok () ⟨F, τ, σ⟩
+    | Except.error τ => Result.error () ⟨F, τ, σ⟩
+  else
+    EStateM.throw () ⟨F, τ, σ⟩
+
+-- Set the witness substitution σ from the provided mapping, resetting σ first
+def assumeWitness (σ : PS) (pivot : ILit) (A₁ : Array ILit) (A₂ : Array (IVar × ILit)) : PS :=
+  ((σ.reset.setLits A₁).setVars A₂).setLit pivot
+
+-- Check each clause in the formula.
+-- C is the current clause in the formula to be checked for the RAT property under σ and τ
+-- If C is reduced by σ, then it is RAT. Find a RAT hint and uses the RAT UP hints to derive contradiction.
+-- (Nat × Nat × Nat) is (ratIndex, index, bumpCounter), where
+--     index := the current index into the formula
+--     ratIndex := the (hopeful, cached) index into the RAT hints
+--     bumpCounter := the number of times we've bumped the assignment
+def checkClause (ratHints : Array (Nat × Array Nat)) :
+    Nat → (Nat × Nat) → ESt CNF Unit (Nat × Nat) := fun index ⟨ratIndex, bumpCounter⟩ => do
+  --let reducedRes ← SRreduce index
+  --let F := dbgTraceIfShared "Formula in checkClause" F
+  St.ebind (SRreduce index) fun v => do
+  match v with
+  | .satisfied => return (ratIndex, bumpCounter)
+  | .notReduced => return (ratIndex, bumpCounter)
+  | _ =>
+    -- We expect a RAT clause. Check if we have bumps left
+    if bumpCounter < ratHints.size then
+      -- Curiously, if the clause is completely falsified, we can still succeed
+      -- on the check (which sr-check does not allow). This is because a UP
+      -- derivation on a completely falsified clause is a global UP derivation,
+      -- and so the certificate can be reduced quite a bit.
+
+      -- Find a RAT hint matching the clause
+      -- We hope that the hints are sorted, but they don't have to be
+      match findRATHintIndex ratIndex index ratHints with
+      | none => EStateM.throw ()
+      | some rI =>
+        -- CC TODO: There's probably an idiomatic way of writing this
+       (fun v =>
+          match v with
+          -- If the clause is satisfied under σ and τ, then we move to the next iteration
+          | Result.error () S =>
+              Result.ok (rI.val + 1, bumpCounter + 1) ({ S with τ := S.τ.bump })
+
+          -- Otherwise, we have assumed the negation of the RAT clause
+          -- Now check for UP derivation through its hints
+          | Result.ok () S =>
+            let ⟨_, hints⟩ := ratHints.get rI
+            (fun v' =>
+              match v' with
+              | Result.error true S =>
+                  Result.ok (rI.val + 1, bumpCounter + 1) ({ S with τ := S.τ.bump })
+              | Result.error false S => Result.error () S
+              | Result.ok _ S => Result.error () S)
+            ∘ hints.foldlM (init := ()) (fun _ hint => applyUPHint 0 hint) <| S
+        ) ∘ (assumeRATClause index)
+
+    -- We error if the bumpCounter equals the number of RAT hints, since that
+    -- means we bumped the assignment too many times, clearing out the
+    -- assumption of the candidate clause
+    else EStateM.throw ()
+
+def checkLine (line : SRLine) : ESt CNF Bool Unit :=
+  --let ⟨F, τ, σ⟩ := dbgTraceIfShared "Formula at start of checkLine" S
+  let ⟨C, w_tf, w_maps, UPhints, RAThints⟩ := line
+
+  -- Assumes the negation of the candidate clause, with "# of RAT hints" offset
+  --modifyGet (fun ⟨F, τ, σ⟩ =>
+  --  match assumeNegatedClauseFor τ.reset C (RAThints.size + 1) with
+  -- Gotta write this as a function, for now
+  fun ⟨F, τ, σ⟩ =>
+  match assumeNegatedClauseFor τ.reset C (RAThints.size + 1) with
+  | Except.error _ => EStateM.throw false ⟨F, τ, σ⟩
+  | Except.ok τ =>
+
+  -- Evaluate the UP hints, with "# of RAT hints" offset
+  -- We add one more than normal to help with proving
+  (fun v =>
+    match v with
+    -- The clause led to contradiction via unit propagation
+    | Result.error true S =>
+      if C = #[] then EStateM.throw true S
+      else ESt.addClause C S
+
+    -- Unit propagation failed due to multiple unassigned literals, satisfied clause, or out-of-bounds
+    | Result.error false S => EStateM.throw false S
+
+    -- Unit propagation worked but didn't lead to contradiction, so continue to RAT checking
+    | Result.ok () ⟨F, τ, σ⟩ =>
+      -- If the clause is empty, then we should have derived UP contradiction by now
+      if hCw : 0 < C.size ∧ 0 < w_tf.size then
+        if C.get ⟨0, hCw.1⟩ ≠ w_tf.get ⟨0, hCw.2⟩ then EStateM.throw false ⟨F, τ, σ⟩ else
+
+        -- Assume the witness, under substitution (the function call resets σ)
+        let σ := assumeWitness σ (C.get ⟨0, hCw.1⟩) w_tf w_maps
+        --let F := dbgTraceIfShared "Formula" F
+
+        -- Go through each clause in the formula to check RAT
+        let Fsize := size F
+        let f := checkClause RAThints
+        let rec loop (i : Nat) (p : Nat × Nat) : ESt CNF Unit (Nat × Nat) := do
+          if i < Fsize then
+            loop (i + 1) (← f i p)
+          else
+            pure p
+          termination_by Fsize - i
+        match loop 0 ⟨0, 0⟩ <| ⟨F, τ, σ⟩ with
+        | Result.error () S => EStateM.throw false S
+        | Result.ok _ S =>
+          --let F := dbgTraceIfShared "Formula at end of checkLine" F
+          ESt.addClause C S -- The RAT hint checked, so we continue
+
+      else EStateM.throw false ⟨F, τ, σ⟩)
+  ∘ UPhints.foldlM (init := ()) (fun _ hint => applyUPHint (RAThints.size + 1) hint) <| ⟨F, τ, σ⟩
+
+
+/-
+def checkProof (F : CNF) (proof : Array SRLine) : Bool :=
+  let τ := PPA.new 100
+  let σ := PS.new 100
+  match proof.foldlM (init := ⟨F, τ, σ⟩) (fun _ S => checkLine S) with
+  | ok _ => false
+  | error false => false
+  | error true => true -/
+
+end SR
