Experiments/ProofChecking/Trash.lean
@@ -1,0 +1,602 @@
+-- CC: An attempt to get parsing faster, given that the Except monad can be expensive
+def parseLSRLine'_aux (pivot : Option ILit) (line : SRAdditionLine) (mode : SRParsingMode) : List String → Except String (SRAdditionLine × SRParsingMode)
+  | [] => ok (line, mode)
+  | atom :: atoms =>
+  -- No matter what, the string should be a number, so parse it as an int
+  match atom.toInt? with
+  | none => throw s!"Atom {atom} didn't parse to a number"
+  | some n =>
+    if hn : n = 0 then
+      match mode with
+      | .clause =>
+        -- We don't have a witness, so we insert the pivot into the witness and continue, if the clause isn't empty
+        match pivot with
+        | none => parseLSRLine'_aux pivot line .upHints atoms
+        | some pivot => parseLSRLine'_aux pivot { line with witnessLits := line.witnessLits.push pivot } .upHints atoms
+      | .witnessLits => parseLSRLine'_aux pivot line .upHints atoms
+      | .witnessMappedReady => parseLSRLine'_aux pivot line .upHints atoms
+      | .witnessMappedHalfway _ => throw s!"Only got half a substitution mapping when ending a witness"
+      | .upHints => parseLSRLine'_aux pivot line .lineDone atoms
+      | .ratHints index hints =>
+          parseLSRLine'_aux pivot { line with
+            ratHintIndexes := line.ratHintIndexes.push index,
+            ratHints := line.ratHints.push hints,
+            ratSizesEq := by simp [line.ratSizesEq] } .lineDone atoms
+      | .lineDone => throw s!"Addition line continued after last ending 0"
+      | .err str => throw str
+    else
+      match mode with
+      | .clause =>
+        match pivot with
+        | none => throw "No pivot provided for the clause"
+        | some pivot =>
+          if n = pivot.val then
+            -- Seeing the pivot again means we're parsing a witness
+            parseLSRLine'_aux pivot { line with witnessLits := line.witnessLits.push ⟨n, hn⟩ } .witnessLits atoms
+          else
+            -- It's not the pivot (and it's not 0), so add it to the clause
+            parseLSRLine'_aux pivot { line with clause := line.clause.push ⟨n, hn⟩ } .clause atoms
+      | .witnessLits =>
+        match pivot with
+        | none => throw "No pivot provided for the witness"
+        | some pivot =>
+          if n = pivot.val then
+            -- Seeing the pivot again means we're parsing the substitution mappings
+            parseLSRLine'_aux pivot line .witnessMappedReady atoms
+          else
+            parseLSRLine'_aux pivot { line with witnessLits := line.witnessLits.push ⟨n, hn⟩ } .witnessLits atoms
+      | .witnessMappedReady =>
+        match pivot with
+        | none => throw "No pivot provided for the witness"
+        | some pivot =>
+          if n = pivot.val then
+            throw s!"Saw pivot again in substitution mapping"
+          else
+            if n < 0 then
+              throw s!"First of a substitution mapping must be positive"
+            else
+              parseLSRLine'_aux pivot line (.witnessMappedHalfway ⟨n.natAbs, Int.natAbs_pos.mpr hn⟩) atoms
+      | .witnessMappedHalfway v =>
+        parseLSRLine'_aux pivot {line with
+          witnessMaps := line.witnessMaps.push v |>.push ⟨n, hn⟩,
+          witnessMapsMod := by simp [add_assoc, Nat.add_mod_right, line.witnessMapsMod] } .witnessMappedReady atoms
+      | .upHints =>
+        if n < 0 then
+          match pivot with
+          | none => throw "Can't have RAT hints for empty clauses"
+          | _ =>
+            -- This is our first RAT hint - start building it
+            parseLSRLine'_aux pivot line (.ratHints (n.natAbs - 1) #[]) atoms
+        else
+          parseLSRLine'_aux pivot { line with upHints := line.upHints.push (n.natAbs - 1) } .upHints atoms
+      | .ratHints index hints =>
+        if n < 0 then
+          -- This is a new RAT hint - add the old one
+          parseLSRLine'_aux pivot { line with
+            ratHintIndexes := line.ratHintIndexes.push index,
+            ratHints := line.ratHints.push hints,
+            ratSizesEq := by simp [line.ratSizesEq] } (.ratHints (n.natAbs - 1) #[]) atoms
+        else
+          parseLSRLine'_aux pivot line (.ratHints index (hints.push (n.natAbs - 1))) atoms
+      | .lineDone => throw s!"Addition line continued after last ending 0"
+      | .err str => throw str
+
+def parseLSRLine' (maxId : Nat) (s : String) : Except String (Nat × (SRAdditionLine ⊕ SRDeletionLine)) :=
+  match s.splitOn " " with
+  | [] => throw "Empty line"
+  | [_] => throw s!"Single atom line: {s}, with id {maxId}"
+  | (id :: hd :: tls) =>
+    match hd with
+    | "d" =>
+      -- Check to make sure the maxId is (non-strictly) monotonically increasing
+      match id.toNat? with
+      | none => throw "Line ID is not a number"
+      | some id =>
+        if id < maxId then
+          throw "Deletion line id is not increasing"
+        else
+          match tls.foldlM (fun arr str =>
+            match str.toNat? with
+            | none => throw (throw s!"{str} was not a number")
+            | some 0 => throw (return arr)
+            | some (n + 1) => return arr.push n) #[] with
+          | ok _ => throw "Zero not found on deletion line"
+          | error e => return ⟨max id maxId, .inr (SRDeletionLine.mk (← e))⟩
+    | _ =>
+      -- We have an addition line, so the maxId should strictly increase
+      match id.toNat? with
+      | none => throw "Line ID is not a number"
+      | some id =>
+        if id ≤ maxId then
+          throw s!"Addition line id is not increasing: parsed {id}, max {maxId}"
+        else
+          match hd.toInt? with
+          | none => throw "Pivot is not a number"
+          | some n =>
+            let line := SRAdditionLine.new
+            if hn : n = 0 then
+              match parseLSRLine'_aux none line .upHints tls with
+              | error str => throw str
+              | ok ⟨line, mode⟩ =>
+                if mode != .lineDone then
+                  throw "Addition line for empty clause didn't end with 0"
+                else
+                  return ⟨id, .inl line⟩
+            else
+              match parseLSRLine'_aux (some ⟨n, hn⟩) { line with clause := line.clause.push ⟨n, hn⟩ } .clause tls with
+              | error str => throw str
+              | ok ⟨line, mode⟩ =>
+                if mode != .lineDone then
+                  throw "Addition line didn't end with 0"
+                else
+                  return ⟨id, .inl line⟩
+
+-- A unit propagation function `UP` is lawful if it returns `MUPResult`s as expected. -/
+def LawfulUP (UP : PPA → IClause → MUPResult) : Prop :=
+  ∀ (τ : PPA) (C : IClause),
+    (UP τ C = .falsified → C.toPropFun ⊓ τ = ⊥)
+  ∧ (∀ {l : ILit}, UP τ C = .unit l →
+        l ∈ C ∧ τ.litValue? l = none ∧ C.toPropFun ⊓ τ ≤ l.toPropFun ⊓ τ)
+  ∧ (UP τ C = .satisfied → τ ≤ C.toPropFun)
+
+theorem LawfulUP_of_eq_of_LawfulUP {UP UP' : PPA → IClause → MUPResult} :
+    (∀ τ C, UP τ C = UP' τ C) → LawfulUP UP → LawfulUP UP' := by
+  intro h_eq h_lawful
+  intro τ C
+  have := h_lawful τ C
+  rw [h_eq τ C] at this
+  exact this
+
+private def pevalM_SatisfiesM_motive (τ : PPA) (C : IClause) : ℕ → Option ILit → Prop
+  | idx, none => ∀ ⦃i : Fin C.size⦄, i < idx → τ.litValue? C[i] = some false
+  | idx, some lit => lit ∈ C.data ∧ τ.litValue? lit = none ∧
+      (∀ ⦃j : Fin C.size⦄, j < idx → C[j] ≠ lit → τ.litValue? C[j] = some false)
+
+theorem foldlM_pevalM_some {τ : PPA} {unit : ILit} :
+  τ.litValue? unit = none → ∀ (C : IClause),
+    ((C.foldlM (pevalM τ) (some unit) = ok (some unit) ∧ C.toPropFun ⊓ τ ≤ unit)
+    ∨ (C.foldlM (pevalM τ) (some unit) = error true ∧ τ ≤ C.toPropFun)
+    ∨ (C.foldlM (pevalM τ) (some unit) = error false)) := by
+  intro h_unit C
+  have ⟨C⟩ := C
+  induction' C with l ls ih generalizing τ
+  · simp [pure, Except.pure]
+  · simp only [Array.foldlM_cons, pevalM]
+    match hl : τ.litValue? l with
+    | none =>
+      by_cases h_eq : l = unit
+      · subst h_eq
+        simp only [↓reduceIte]
+        rcases ih h_unit with (⟨h₁, h₂⟩ | ⟨h₁, h₂⟩ | h)
+        · left; use h₁
+          rw [Clause.toPropFun_cons, inf_sup_right]
+          exact sup_le inf_le_left h₂
+        · right; left; use h₁
+          rw [Clause.toPropFun_cons]
+          exact le_trans h₂ le_sup_right
+        · right; right; use h
+      · simp [Ne.symm h_eq]; right; right; rfl
+    | some true =>
+      right; left; use rfl
+      rw [litValue?_true_iff] at hl
+      rw [Clause.toPropFun_cons]
+      exact le_trans hl le_sup_left
+    | some false =>
+      rcases ih h_unit with (⟨h₁, h₂⟩ | ⟨h₁, h₂⟩ | h)
+      · left; use h₁
+        rw [litValue?_false_iff, le_compl_iff_inf_le_bot, le_bot_iff, inf_comm] at hl
+        simp [Clause.toPropFun_cons, inf_sup_right, hl, h₂]
+      · right; left; use h₁
+        rw [Clause.toPropFun_cons]
+        exact le_trans h₂ le_sup_right
+      · right; right; use h
+
+theorem unitPropM_LawfulUP : LawfulUP unitPropM := by
+  rintro τ ⟨C⟩
+  induction' C with l ls ih generalizing τ
+  · simp [unitPropM, pure, Except.pure]
+  · rw [unitPropM, Array.foldlM_cons, pevalM]
+    match hl : τ.litValue? l with
+    | none =>
+      simp only
+      rcases foldlM_pevalM_some hl { data := ls } with (⟨h₁, h₂⟩ | ⟨h₁, h₂⟩ | h)
+      · split
+        <;> rename _ => h_cons
+        <;> try simp only [bind, Except.bind, h₁] at h_cons
+        <;> injection h_cons
+        · contradiction
+        · rename _ => h_lit; injection h_lit; rename _ => h_lit; subst h_lit
+          simp [← Array.mem_data, hl, inf_sup_right, h₂]
+      · split
+        <;> rename _ => h_cons
+        <;> try simp only [bind, Except.bind, h₁] at h_cons
+        · simp; exact le_sup_of_le_right h₂
+        · injection h_cons; contradiction
+      · split
+        <;> rename _ => h_cons
+        <;> try simp only [bind, Except.bind, h] at h_cons
+        <;> injection h_cons
+        · contradiction
+        · simp
+    | some true =>
+      simp [bind, Except.bind]
+      rw [litValue?_true_iff] at hl
+      exact le_sup_of_le_left hl
+    | some false =>
+      simp only [bind, Except.bind]
+      rcases ih τ with ⟨h₁, h₂, h₃⟩
+      rw [litValue?_false_iff, le_compl_iff_inf_le_bot, le_bot_iff, inf_comm] at hl
+      split
+      <;> rename _ => h_cons
+      · simp only [unitPropM, h_cons, forall_true_left] at h₁
+        simp [inf_sup_right, hl, h₁]
+      · rename ILit => l'
+        simp only [unitPropM, h_cons, forall_true_left] at h₂
+        replace h₂ := @h₂ l'
+        simp at h₂
+        rcases h₂ with ⟨h_mem, hτl', h_le⟩
+        simp [← Array.mem_data] at h_mem ⊢
+        use Or.inr h_mem, hτl'
+        simp [inf_sup_right, h_le, hl]
+      · simp only [unitPropM, h_cons, forall_true_left] at h₃
+        simp [le_sup_of_le_right h₃]
+      · simp
+
+#exit
+
+theorem unitPropM_LawfulUP : LawfulUP unitPropM := by
+  intro τ C
+  have h_SM := C.SatisfiesM_foldlM (init := (none : Option ILit)) (f := pevalM τ)
+    (motive := pevalM_SatisfiesM_motive τ C)
+    (h0 := by simp [pevalM_SatisfiesM_motive])
+    (hf := by
+      unfold pevalM_SatisfiesM_motive
+      simp only [SatisfiesM_Except_eq, getElem_fin]
+      intro i box ih
+        -- CC: Is this proof more compact if I use pattern-matching with intro?
+      intro
+      | none, hbox =>
+        intro j hj
+        unfold pevalM at hbox
+        cases h_tau : τ.litValue? C[i.val] with
+        | none =>
+          simp [h_tau] at hbox
+          cases h_box : box with
+          | none => simp [h_box] at hbox
+          | some lit => by_cases h_lit : lit = C[i.val] <;> simp [h_box, h_lit] at hbox
+        | some b =>
+          cases h_box : box with
+          | none =>
+            subst h_box
+            rcases lt_or_eq_of_le (le_of_lt_succ hj) with (h | h)
+            · exact ih h
+            · cases b
+              · replace h := Fin.ext h; subst h; exact h_tau
+              · simp [h_tau] at hbox
+          | some lit => by_cases h_lit : lit = C[i.val] <;> cases b <;> simp [h_tau, h_box, h_lit] at hbox
+      | some lit, hbox =>
+        unfold pevalM at hbox
+        cases h_tau : τ.litValue? C[i.val] with
+        | none =>
+          simp [h_tau] at hbox
+          cases h_box : box with
+          | none =>
+            subst h_box
+            simp at hbox
+            use Array.mem_data_iff_exists_fin.mpr ⟨i, hbox⟩, hbox ▸ h_tau
+            intro j hj₁ hj₂
+            rcases lt_or_eq_of_le (le_of_lt_succ hj₁) with (h | h)
+            · exact ih h
+            · simp at ih
+              replace h := Fin.ext h; subst h; rw [hbox] at hj₂; contradiction
+          | some l =>
+            subst h_box
+            by_cases hl : l = C[i.val]
+            · simp [hl] at hbox
+              rw [hbox] at hl
+              subst hl
+              rcases ih with ⟨hl₁, hl₂, ih⟩
+              use hl₁, hl₂
+              intro j hj₁ hj₂
+              rcases lt_or_eq_of_le (le_of_lt_succ hj₁) with (h | h)
+              · exact ih h hj₂
+              · replace h := Fin.ext h; subst h; rw [hbox] at hj₂; contradiction
+            · simp [hl] at hbox
+        | some b =>
+          cases b
+          · simp [h_tau] at hbox
+            subst hbox
+            rcases ih with ⟨hlit₁, hlit₂, ih⟩
+            use hlit₁, hlit₂
+            intro j hj₁ hj₂
+            rcases lt_or_eq_of_le (le_of_lt_succ hj₁) with (h | h)
+            · exact ih h hj₂
+            · replace h := Fin.ext h; subst h; exact h_tau
+          · simp [h_tau] at hbox)
+  unfold unitPropM
+  match hUP : C.foldlM (pevalM τ) none with
+  | ok none =>
+    simp
+    have := SatisfiesM_Except_eq.mp h_SM none hUP
+    simp [pevalM_SatisfiesM_motive, -getElem_fin] at this
+    rw [← le_bot_iff]
+    refine entails_ext.mpr fun τ' hτ' => ?_
+    -- CC: Is there a way to do this with a single tactic?
+    rw [satisfies_conj] at hτ'; rcases hτ' with ⟨hττ', hCτ'⟩
+    rw [Clause.satisfies_iff] at hCτ'; rcases hCτ' with ⟨lit, hlit, hτ'lit⟩
+    rw [← Array.mem_data] at hlit
+    rcases Array.mem_data_iff_exists_fin.mp hlit with ⟨i, hi⟩
+    have := @this i
+    rw [hi, litValue?_false_iff] at this
+    exact absurd hτ'lit (PropFun.satisfies_neg.mp (entails_ext.mp this τ' hττ'))
+  | ok (some lit) =>
+    simp
+    have := SatisfiesM_Except_eq.mp h_SM (some lit) hUP
+    simp [pevalM_SatisfiesM_motive, -getElem_fin] at this
+    rcases this with ⟨hlit₁, hlit₂, hlit₃⟩
+    rw [← Array.mem_data]
+    use hlit₁, hlit₂
+    refine entails_ext.mpr fun τ' hτ' => ?_
+    rw [satisfies_conj] at hτ'; rcases hτ' with ⟨hCτ', hττ'⟩
+    rw [Clause.satisfies_iff] at hCτ'; rcases hCτ' with ⟨lit', hlit', hτ'lit'⟩
+    by_cases hlits_eq : lit = lit'
+    · subst hlits_eq
+      exact hτ'lit'
+    · rw [← Array.mem_data] at hlit'
+      rcases Array.mem_data_iff_exists_fin.mp hlit' with ⟨i, rfl⟩
+      have := hlit₃ (Ne.symm hlits_eq)
+      rw [← litValue?_negate_some_iff', Bool.not_false] at this
+      rw [satisfies_iff_lits] at hττ'
+      have := hττ' this
+      rw [toPropFun_neg, PropFun.satisfies_neg] at this
+      exact absurd hτ'lit' this
+  | error true => simp
+  | error false => simp
+
+theorem unitProp_LawfulUP (s e : Nat) : LawfulUP (unitProp' s e) := by
+  refine LawfulUP_of_eq_of_LawfulUP ?_ unitPropM_LawfulUP
+  intro τ C
+
+  done
+
+#exit
+ /-
+   unfold unitProp unitPropRes
+  intro h_falsified
+  split at h_falsified
+  <;> try simp at h_falsified
+  clear h_falsified
+  rename (foldUP τ C = ok none) => h
+  refine entails_ext.mpr fun τ' hτ' => ?_
+  rw [satisfies_conj] at hτ'
+  rcases hτ' with ⟨hττ', hCτ'⟩
+  have ⟨lit, hlit, hτ'lit⟩ := Clause.satisfies_iff.mp hCτ'
+  rw [← Array.mem_data] at hlit
+  have hlv := SatisfiesM_Except_eq.mp (SatisfiesM_UP τ C) none h lit hlit
+  clear h hCτ' hlit
+  have := satisfies_iff_vars.mp hττ'
+  replace hτ'lit := LitVar.satisfies_iff.mp hτ'lit
+  cases hpol : polarity lit
+  <;> simp [hpol] at hτ'lit
+  <;> simp [litValue?, hpol] at hlv
+  <;> rw [this hlv] at hτ'lit
+  <;> contradiction
+ -/
+  --unfold unitPropM
+  --suffices
+  generalize h_unit? : none = unit?
+  induction' C with l ls ih generalizing τ unit?
+  · simp [unitPropM, pure, Except.pure, ← h_unit?]
+  · match hl : τ.litValue? l with
+    | none =>
+      done
+
+    done
+  done
+
+#exit
+
+/-- The "Bool" is true if satisfied, false if not. -/
+def pevalUP (τ : PPA) (unit? : Option ILit) (l : ILit) : Except Bool (Option ILit) :=
+  match τ.litValue? l with
+  | some true => error true
+  | some false => ok unit?
+  | none =>
+    match unit? with
+    | none => ok l
+    | some u =>
+      if u = l then ok unit?
+      -- Assume tautology cannot occur in clause, so two unassiged literals exits early
+      else error false
+
+def foldUP (τ : PPA) (C : IClause) := C.foldlM (pevalUP τ) none
+
+def unitPropRes (res : Except Bool (Option ILit)) : MUPResult :=
+  match res with
+  | ok none => .falsified
+  | ok (some lit) => .unit lit
+  | error true => .satisfied
+  | error false => .multipleUnassignedLiterals
+
+def unitProp (τ : PPA) (C : IClause) : MUPResult :=
+  unitPropRes (foldUP τ C)
+
+-- Alternate view of unit propagation, using indexes into an array
+def unitPropOnIndexes (τ : PPA) (C : IClause) (s e : Nat) : MUPResult :=
+  let min_e := min e C.size
+  let rec go (i : Nat) (unit? : Option ILit) : MUPResult :=
+    if hi : i < min_e then
+      -- This is essentially a clone of `pevalUP` above, except without an Exception monad
+      let lit := C.get ⟨i, Nat.lt_of_lt_of_le hi (min_le_right e C.size)⟩
+      match τ.litValue? lit with
+      | some true => .satisfied
+      | some false => go (i + 1) unit?
+      | none =>
+        match unit? with
+        | none => go (i + 1) (some lit)
+        | some u =>
+          if u = lit then go (i + 1) unit?
+          else .multipleUnassignedLiterals
+    else
+      match unit? with
+      | none => .falsified
+      | some l => .unit l
+  termination_by (min e C.size) - i
+  go s none
+
+
+
+
+#exit
+
+
+
+theorem SatisfiesM_UP (τ : PPA) (C : IClause) :
+    SatisfiesM (fun
+      -- If there are no unassigned literals, then all should be false
+      | none => ∀ l ∈ C.data, τ.litValue? l = some false
+      | some lit => lit ∈ C.data ∧ τ.litValue? lit = none ∧
+          (∀ l ∈ C.data, l ≠ lit → τ.litValue? l = some false)) (foldUP τ C) := by
+  have := C.SatisfiesM_foldlM (init := (none : Option ILit)) (f := pevalUP τ)
+    (motive := motive_fn τ C)
+    (h0 := by simp [motive_fn]) -- Why do I have to define it right above? Putting it inline with (motive :=) had sorryAx problems
+    (hf := by
+      unfold motive_fn
+      simp only [SatisfiesM_Except_eq, getElem_fin]
+      intro i box ih
+        -- Cayden question: Is this proof more compact if I use pattern-matching with intro?
+      intro
+      | none, hbox =>
+        intro j hj
+        unfold pevalUP at hbox
+        cases h_tau : τ.litValue? C[i.val] with
+        | none =>
+          simp [h_tau] at hbox
+          cases h_box : box with
+          | none => simp [h_box] at hbox
+          | some lit => by_cases h_lit : lit = C[i.val] <;> simp [h_box, h_lit] at hbox
+        | some b =>
+          cases h_box : box with
+          | none =>
+            subst h_box
+            rcases lt_or_eq_of_le (le_of_lt_succ hj) with (h | h)
+            · exact ih h
+            · cases b
+              · replace h := Fin.ext h; subst h; exact h_tau
+              · simp [h_tau] at hbox
+          | some lit => by_cases h_lit : lit = C[i.val] <;> cases b <;> simp [h_tau, h_box, h_lit] at hbox
+      | some lit, hbox =>
+        unfold pevalUP at hbox
+        cases h_tau : τ.litValue? C[i.val] with
+        | none =>
+          simp [h_tau] at hbox
+          cases h_box : box with
+          | none =>
+            subst h_box
+            simp at hbox
+            use Array.mem_data_iff_exists_fin.mpr ⟨i, hbox⟩, hbox ▸ h_tau
+            intro j hj₁ hj₂
+            rcases lt_or_eq_of_le (le_of_lt_succ hj₁) with (h | h)
+            · exact ih h
+            · simp at ih
+              replace h := Fin.ext h; subst h; rw [hbox] at hj₂; contradiction
+          | some l =>
+            subst h_box
+            by_cases hl : l = C[i.val]
+            · simp [hl] at hbox
+              rw [hbox] at hl
+              subst hl
+              rcases ih with ⟨hl₁, hl₂, ih⟩
+              use hl₁, hl₂
+              intro j hj₁ hj₂
+              rcases lt_or_eq_of_le (le_of_lt_succ hj₁) with (h | h)
+              · exact ih h hj₂
+              · replace h := Fin.ext h; subst h; rw [hbox] at hj₂; contradiction
+            · simp [hl] at hbox
+        | some b =>
+          cases b
+          · simp [h_tau] at hbox
+            subst hbox
+            rcases ih with ⟨hlit₁, hlit₂, ih⟩
+            use hlit₁, hlit₂
+            intro j hj₁ hj₂
+            rcases lt_or_eq_of_le (le_of_lt_succ hj₁) with (h | h)
+            · exact ih h hj₂
+            · replace h := Fin.ext h; subst h; exact h_tau
+          · simp [h_tau] at hbox)
+  apply SatisfiesM.imp this
+  intro
+  | none =>
+    intro h l hl
+    rcases Array.mem_data_iff_exists_fin.mp hl with ⟨i, rfl⟩
+    exact h i.isLt
+  | some lit =>
+    simp [motive_fn]
+    intro hlit₁ hlit₂ ih
+    use hlit₁, hlit₂
+    intro l hl₁ hl₂
+    rcases Array.mem_data_iff_exists_fin.mp hl₁ with ⟨i, rfl⟩
+    exact ih hl₂
+
+-- Cayden TODO/Q: Allow for [pattern_match] on ResultT? What is [unbox]?
+-- Cayden Q: when aesop can't solve something, why does [aesop?] not give anything?
+theorem contradiction_of_UP_falsified {τ : PPA} {C : IClause} :
+    τ.unitProp C = .falsified → τ.toPropFun ⊓ C.toPropFun ≤ ⊥ := by
+  unfold unitProp unitPropRes
+  intro h_falsified
+  split at h_falsified
+  <;> try simp at h_falsified
+  clear h_falsified
+  rename (foldUP τ C = ok none) => h
+  refine entails_ext.mpr fun τ' hτ' => ?_
+  rw [satisfies_conj] at hτ'
+  rcases hτ' with ⟨hττ', hCτ'⟩
+  have ⟨lit, hlit, hτ'lit⟩ := Clause.satisfies_iff.mp hCτ'
+  rw [← Array.mem_data] at hlit
+  have hlv := SatisfiesM_Except_eq.mp (SatisfiesM_UP τ C) none h lit hlit
+  clear h hCτ' hlit
+  have := satisfies_iff_vars.mp hττ'
+  replace hτ'lit := LitVar.satisfies_iff.mp hτ'lit
+  cases hpol : polarity lit
+  <;> simp [hpol] at hτ'lit
+  <;> simp [litValue?, hpol] at hlv
+  <;> rw [this hlv] at hτ'lit
+  <;> contradiction
+
+-- Is it better to say that ¬(τ ≤ l), or that τ.litValue? l = none?
+theorem extended_of_UP_unit {τ : PPA} {C : IClause} {l : ILit} :
+    τ.unitProp C = .unit l →
+      l ∈ C ∧
+      τ.litValue? l = none ∧
+      C.toPropFun ⊓ τ.toPropFun ≤ l.toPropFun ⊓ τ := by
+  unfold unitProp unitPropRes
+  intro h_unit
+  split at h_unit
+  <;> try simp at h_unit
+  rename ILit => lit; subst h_unit
+  rename (foldUP τ C = ok (some lit)) => h
+  have hlv := SatisfiesM_Except_eq.mp (SatisfiesM_UP τ C) (some lit) h
+  clear h
+  rcases hlv with ⟨hlit, hτlit, ih⟩
+  rw [← Array.mem_data]
+  use hlit, hτlit
+  refine entails_ext.mpr fun τ' hτ' => ?_
+  rw [satisfies_conj] at hτ'; rcases hτ' with ⟨hCτ', hττ'⟩
+  rw [satisfies_iff_lits] at hττ'
+  rw [Clause.satisfies_iff] at hCτ'; rcases hCτ' with ⟨m, hm, hmτ'⟩
+  by_cases heq : m = lit
+  · subst heq
+    rw [← satisfies_iff_lits] at hττ'
+    rw [satisfies_conj]
+    exact ⟨hmτ', hττ'⟩
+  · rw [← Array.mem_data] at hm
+    replace ih := ih _ hm heq
+    have := litValue?_negate τ m
+    simp only [ih, Option.map_some', Bool.not_false] at this
+    have := hττ' this
+    simp at this
+    exact absurd hmτ' this
+
+end monadic /- section -/
+
+end PPA
